clightlight/Clightlight2ClightSim.v
@@ -10,7 +10,6 @@ Require Import ConvC2ITree.
 Require Import SimSTS3.
 Require Import Clight_Mem0.
 Require Import IRed.
-From Ordinal Require Import Ordinal Arithmetic.
 
 Require Import Clightlight2ClightMatch.
 Require Import Clightlight2ClightArith.
@@ -63,7 +62,7 @@ Section PROOF.
   Hint Resolve _sim_mon: paco.
 
   Ltac sim_red := try red; Red.prw ltac:(_red_gen) 2 0.
-  Ltac sim_tau := (try sim_red); pfold; econs 3; ss; clarify; eexists; exists (step_tau _); left.
+  Ltac sim_tau := (try sim_red); try pfold; econs 3; ss; clarify; eexists; exists (step_tau _).
 
   Definition arrow (A B: Prop): Prop := A -> B.
   Opaque arrow.
@@ -98,15 +97,16 @@ Section PROOF.
 
   Ltac solve_ub := des; irw in H; dependent destruction H; clarify.
   Ltac sim_triggerUB := 
-    (try rename H into HH); ss; unfold triggerUB; try sim_red; pfold; econs 5; i; ss; auto;
+    (try rename H into HH); ss; unfold triggerUB; try sim_red; try pfold; econs 5; i; ss; auto;
                         [solve_ub | irw in  STEP; dependent destruction STEP; clarify].
 
-  Ltac tgt_step := pfold; econs 4; eexists; eexists; [|left].
+  Ltac tgt_step := try pfold; econs 4; eexists; eexists; [|left].
 
-  Ltac wrap_up := pfold; econs 7; et; right.
+  Ltac wrap_up := try pfold; econs 7; et; right.
 
   Ltac remove_UBcase := des_ifs; try sim_red; try sim_triggerUB.
 
+  Ltac eapplyf NEXT := let X := fresh "X" in hexploit NEXT;[..|intro X; punfold X; et].
   Ltac dtm H H0 := eapply angelic_step in H; eapply angelic_step in H0; des; rewrite H; rewrite H0; ss.
 
   Local Opaque Pos.of_nat.
@@ -138,10 +138,12 @@ Section PROOF.
           pstate);; ktr r0)
       (State tf tcode tcont te tle tm).
   Proof.
-    unfold ccallU. sim_red. sim_tau. ss. sim_red. unfold loadF. repeat (sim_red; sim_tau). sim_red.
+    unfold ccallU. sim_red. 
+    sim_tau. ss. sim_red. unfold loadF. repeat (sim_red; sim_tau). sim_red.
     rewrite PSTATE. sim_red. unfold unwrapU. remove_UBcase. sim_tau. sim_red. rewrite Any.upcast_downcast.
-    sim_red. eapply NEXT. unfold Mem.loadv in *. des_ifs_safe. ss. clarify. hexploit match_mem_load; et.
+    sim_red. eapplyf NEXT. unfold Mem.loadv in *. des_ifs_safe. ss. clarify. hexploit match_mem_load; et.
   Qed.
+  
     
 
   Lemma step_store pstate f_table modl cprog sk tge le tle e te m tm
@@ -172,7 +174,7 @@ Section PROOF.
   Proof.
     unfold ccallU. sim_red. sim_tau. ss. sim_red. unfold storeF. sim_red. repeat (sim_tau; sim_red).
     rewrite PSTATE. sim_red. unfold unwrapU. remove_UBcase. repeat (sim_tau; sim_red). rewrite Any.upcast_downcast.
-    sim_red. unfold Mem.storev in Heq. des_ifs_safe. hexploit match_mem_store; et. i. des. eapply NEXT; et. 
+    sim_red. unfold Mem.storev in Heq. des_ifs_safe. hexploit match_mem_store; et. i. des. eapplyf NEXT; et. 
   Qed.
 
   Lemma step_loadbytes pstate f_table modl cprog sk tge le tle e te m tm
@@ -202,7 +204,7 @@ Section PROOF.
   Proof.
     unfold ccallU. sim_red. sim_tau. ss. sim_red. unfold loadbytesF. repeat (sim_red; sim_tau). sim_red.
     rewrite PSTATE. sim_red. unfold unwrapU. remove_UBcase. sim_tau. sim_red. rewrite Any.upcast_downcast.
-    sim_red. eapply NEXT. hexploit match_mem_loadbytes; et.
+    sim_red. eapplyf NEXT. hexploit match_mem_loadbytes; et.
   Qed.
 
   Lemma step_storebytes pstate f_table modl cprog sk tge le tle e te m tm
@@ -233,7 +235,7 @@ Section PROOF.
   Proof.
     unfold ccallU. sim_red. sim_tau. ss. sim_red. unfold storebytesF. sim_red. repeat (sim_tau; sim_red).
     rewrite PSTATE. sim_red. unfold unwrapU. remove_UBcase. repeat (sim_tau; sim_red). rewrite Any.upcast_downcast.
-    sim_red. hexploit match_mem_storebytes; et. i. des. eapply NEXT; et.
+    sim_red. hexploit match_mem_storebytes; et. i. des. eapplyf NEXT; et.
   Qed.
 
   Lemma step_load_bitfield pstate f_table modl cprog sk tge le tle e te m tm
@@ -263,7 +265,7 @@ Section PROOF.
   Proof.
     unfold load_bitfield_c.
     remove_UBcase; eapply step_load; et;
-      i; remove_UBcase; eapply NEXT; econs; try nia; try des_ifs.
+      i; remove_UBcase; eapplyf NEXT; econs; try nia; try des_ifs.
   Qed.
 
   Lemma step_store_bitfield pstate f_table modl cprog sk tge le tle e te m tm
@@ -295,7 +297,7 @@ Section PROOF.
     unfold store_bitfield_c. remove_UBcase;
       eapply step_load; et; i; remove_UBcase; 
         eapply step_store; et; i; sim_red;
-          eapply NEXT; et; econs; et; try nia; des_ifs.
+          eapplyf NEXT; et; econs; et; try nia; des_ifs.
   Qed.
 
   Lemma step_weak_valid_pointer pstate f_table modl cprog sk tge le tle e te m tm
@@ -325,7 +327,7 @@ Section PROOF.
     unfold weak_valid_pointer_c, ccallU. sim_red. sim_tau. ss. unfold valid_pointerF. sim_red. 
     repeat (sim_tau; sim_red). rewrite PSTATE. sim_red. repeat (sim_tau; sim_red).
     unfold valid_pointerF. sim_red. repeat (sim_tau; sim_red). rewrite PSTATE.
-    sim_red. repeat (sim_tau; sim_red). eapply NEXT; et.
+    sim_red. repeat (sim_tau; sim_red). eapplyf NEXT; et.
     unfold Mem.weak_valid_pointer, Mem.valid_pointer. inv MM.
     repeat (match goal with | |- context ctx [ Mem.perm_dec ?x ] => destruct (Mem.perm_dec x) end); et;
       ss; unfold Mem.perm in *; rewrite <- MEM_PERM in *; contradiction.
@@ -357,9 +359,9 @@ Section PROOF.
       (State tf tcode tcont te tle tm).
   Proof.
     unfold sem_cast_c. des_ifs_safe. des_ifs.
-    all: try solve [sim_red; eapply NEXT; i; clarify; ss; unfold Cop.sem_cast; des_ifs].
+    all: try solve [sim_red; eapplyf NEXT; i; clarify; ss; unfold Cop.sem_cast; des_ifs].
     sim_red. eapply step_weak_valid_pointer; et. i. 
-      des_ifs; sim_red; eapply NEXT; et; ss; i; clarify;
+      des_ifs; sim_red; eapplyf NEXT; et; ss; i; clarify;
        unfold Cop.sem_cast; rewrite Heq1; des_ifs_safe. 
   Qed.
 
@@ -397,17 +399,17 @@ Section PROOF.
       (State tf tcode tcont te tle tm).
   Proof.
     unfold assign_loc_c. des_ifs; try sim_red; try sim_triggerUB.
-    2,3,6,7 : eapply step_store_bitfield; et; i; sim_red; eapply NEXT; et; econs; et.
-    - eapply step_store; et. i. des. eapply NEXT; et. econs; et. 
+    2,3,6,7 : eapply step_store_bitfield; et; i; sim_red; eapplyf NEXT; et; econs; et.
+    - eapply step_store; et. i. des. eapplyf NEXT; et. econs; et. 
     - eapply step_loadbytes; et. i. eapply step_storebytes; et. i.
-      eapply NEXT; et. destruct (_ && _) eqn: E in Heq0; clarify.
+      eapplyf NEXT; et. destruct (_ && _) eqn: E in Heq0; clarify.
       apply andb_true_iff in E. des. econs 2; et; i.
       1,2: rewrite <- divide_c_divides; et; pose proof alignof_blockcopy_pos; et.
       destruct (_||_) eqn: E1 in Heq1 ; clarify. repeat rewrite orb_true_iff in E1.  
       des; try nia. left. destruct (b0 =? blk)%positive eqn:E2 in E1; clarify.
       apply Pos.eqb_neq in E2. red. i. apply E2. eapply map_blk_inj; et; admit "".
     - eapply step_loadbytes; et. i. eapply step_storebytes; et. i.
-      eapply NEXT; et. econs 2; et; i; try nia.
+      eapplyf NEXT; et. econs 2; et; i; try nia.
   Qed.
 
   Lemma step_deref_loc pstate f_table modl cprog sk tge le tle e te m tm
@@ -437,10 +439,10 @@ Section PROOF.
   Proof.
     unfold deref_loc_c. destruct bf.
     - remove_UBcase.
-      + eapply step_load; et. i. eapply NEXT; ss; econs; et.
-      + eapply NEXT; ss; econs 2; et.
-      + eapply NEXT; ss; econs 3; et.
-    - des_ifs; eapply step_load_bitfield; et; i; eapply NEXT; econs; ss.
+      + eapply step_load; et. i. eapplyf NEXT; ss; econs; et.
+      + eapplyf NEXT; ss; econs 2; et.
+      + eapplyf NEXT; ss; econs 3; et.
+    - des_ifs; eapply step_load_bitfield; et; i; eapplyf NEXT; econs; ss.
   Qed.
 
   (* Lemma sk_In sk s n : SkEnv.id2blk (Sk.load_skenv sk) s = Some n -> In s (List.map fst sk).
@@ -479,17 +481,19 @@ Section PROOF.
   Proof.
     unfold unary_op_c. des_ifs; sim_red.
     - unfold bool_val_c. des_ifs.
-      all: try (sim_red; eapply NEXT; i; clarify; ss; unfold Cop.sem_unary_operation; des_ifs; 
-                unfold Cop.sem_notbool, Cop.bool_val; des_ifs).
+      all: try solve [sim_red; eapplyf NEXT; i; clarify; ss; unfold Cop.sem_unary_operation; des_ifs; 
+                unfold Cop.sem_notbool, Cop.bool_val; des_ifs].
       all: try (unfold Values.Val.of_bool; ss; des_ifs).
+      1,2,4,5: sim_red; eapplyf NEXT; i; clarify; ss; unfold Cop.sem_unary_operation; des_ifs; 
+                unfold Cop.sem_notbool, Cop.bool_val; des_ifs; bsimpl; clarify.
       sim_red. eapply step_weak_valid_pointer; et. i. 
-      destruct b1; sim_red; eapply NEXT; et; i; clarify;
+      destruct b1; sim_red; eapplyf NEXT; et; i; clarify;
         unfold Cop.sem_notbool, Cop.bool_val; des_ifs.
-    - eapply NEXT; i;
+    - eapplyf NEXT; i;
         unfold Cop.sem_unary_operation, Cop.sem_notint in *; des_ifs; ss; clarify.
-    - eapply NEXT; i;
+    - eapplyf NEXT; i;
         unfold Cop.sem_unary_operation, Cop.sem_neg in *; des_ifs; ss; clarify.
-    - eapply NEXT; i;
+    - eapplyf NEXT; i;
         unfold Cop.sem_unary_operation, Cop.sem_absfloat in *; des_ifs; ss; clarify.
   Qed.
 
@@ -521,106 +525,106 @@ Section PROOF.
   Proof.
     unfold binary_op_c. des_ifs; unfold sem_add_c, sem_sub_c, sem_mul_c, sem_div_c, sem_mod_c, sem_and_c, sem_or_c, sem_xor_c, Cop.sem_shl, Cop.sem_shr, sem_cmp_c; try sim_red.
     - des_ifs; try sim_red;
-        try (eapply NEXT; i; ss;
+        try (eapplyf NEXT; i; ss;
             unfold Cop.sem_add; rewrite Heq; unfold Cop.sem_add_ptr_int, Cop.sem_add_ptr_long in *; 
             des_ifs; ss; clarify).
       unfold sem_binarith_c. sim_red. eapply step_sem_cast; et. i. destruct optv; sim_red;
-        try solve [eapply NEXT; i; clarify; unfold Cop.sem_binary_operation, Cop.sem_add; rewrite Heq; unfold Cop.sem_binarith;
+        try solve [eapplyf NEXT; i; clarify; unfold Cop.sem_binary_operation, Cop.sem_add; rewrite Heq; unfold Cop.sem_binarith;
                   try (erewrite H by et); try (erewrite H0 by et); try (erewrite H1 by et); try (erewrite H2 by et); ss].
       eapply step_sem_cast; et. i. destruct optv; try sim_red;
-        try solve [eapply NEXT; i; clarify; unfold Cop.sem_binary_operation, Cop.sem_add; rewrite Heq; unfold Cop.sem_binarith;
+        try solve [eapplyf NEXT; i; clarify; unfold Cop.sem_binary_operation, Cop.sem_add; rewrite Heq; unfold Cop.sem_binarith;
                   try (erewrite H by et); try (erewrite H0 by et); try (erewrite H1 by et); try (erewrite H2 by et); ss].
       des_ifs; sim_red; 
-        eapply NEXT; i; clarify; unfold Cop.sem_binary_operation, Cop.sem_add; rewrite Heq; unfold Cop.sem_binarith; 
+        eapplyf NEXT; i; clarify; unfold Cop.sem_binary_operation, Cop.sem_add; rewrite Heq; unfold Cop.sem_binarith; 
           rewrite Heq0 in *; try (erewrite H by et); try (erewrite H0 by et); try (erewrite H1 by et); try (erewrite H2 by et); ss.
     - des_ifs; try sim_red;
-        try (eapply NEXT; i; ss; unfold Cop.sem_sub; rewrite Heq; des_ifs; ss; clarify).
+        try (eapplyf NEXT; i; ss; unfold Cop.sem_sub; rewrite Heq; des_ifs; ss; clarify).
       + eapply map_blk_inj in e0; et. contradiction.
       + 
       unfold sem_binarith_c. sim_red. eapply step_sem_cast; et. i. destruct optv; sim_red;
-        try solve [eapply NEXT; i; clarify; unfold Cop.sem_binary_operation, Cop.sem_sub; rewrite Heq; unfold Cop.sem_binarith;
+        try solve [eapplyf NEXT; i; clarify; unfold Cop.sem_binary_operation, Cop.sem_sub; rewrite Heq; unfold Cop.sem_binarith;
                   try (erewrite H by et); try (erewrite H0 by et); try (erewrite H1 by et); try (erewrite H2 by et); ss].
       eapply step_sem_cast; et. i. destruct optv; try sim_red;
-        try solve [eapply NEXT; i; clarify; unfold Cop.sem_binary_operation, Cop.sem_sub; rewrite Heq; unfold Cop.sem_binarith;
+        try solve [eapplyf NEXT; i; clarify; unfold Cop.sem_binary_operation, Cop.sem_sub; rewrite Heq; unfold Cop.sem_binarith;
                   try (erewrite H by et); try (erewrite H0 by et); try (erewrite H1 by et); try (erewrite H2 by et); ss].
       des_ifs; sim_red; 
-        eapply NEXT; i; clarify; unfold Cop.sem_binary_operation, Cop.sem_sub; rewrite Heq; unfold Cop.sem_binarith; 
+        eapplyf NEXT; i; clarify; unfold Cop.sem_binary_operation, Cop.sem_sub; rewrite Heq; unfold Cop.sem_binarith; 
           rewrite Heq0 in *; try (erewrite H by et); try (erewrite H0 by et); try (erewrite H1 by et); try (erewrite H2 by et); ss.
     - unfold sem_binarith_c. sim_red. eapply step_sem_cast; et. i. destruct optv; sim_red;
-        try solve [eapply NEXT; i; clarify; unfold Cop.sem_binary_operation, Cop.sem_mul; unfold Cop.sem_binarith;
+        try solve [eapplyf NEXT; i; clarify; unfold Cop.sem_binary_operation, Cop.sem_mul; unfold Cop.sem_binarith;
                   try (erewrite H by et); try (erewrite H0 by et); try (erewrite H1 by et); try (erewrite H2 by et); ss].
       eapply step_sem_cast; et. i. destruct optv; try sim_red;
-        try solve [eapply NEXT; i; clarify; unfold Cop.sem_binary_operation, Cop.sem_mul; unfold Cop.sem_binarith;
+        try solve [eapplyf NEXT; i; clarify; unfold Cop.sem_binary_operation, Cop.sem_mul; unfold Cop.sem_binarith;
                   try (erewrite H by et); try (erewrite H0 by et); try (erewrite H1 by et); try (erewrite H2 by et); ss].
       des_ifs; sim_red; 
-        eapply NEXT; i; clarify; unfold Cop.sem_binary_operation, Cop.sem_mul; unfold Cop.sem_binarith; 
+        eapplyf NEXT; i; clarify; unfold Cop.sem_binary_operation, Cop.sem_mul; unfold Cop.sem_binarith; 
           rewrite Heq in *; try (erewrite H by et); try (erewrite H0 by et); try (erewrite H1 by et); try (erewrite H2 by et); ss.
     - unfold sem_binarith_c. sim_red. eapply step_sem_cast; et. i. destruct optv; sim_red;
-        try solve [eapply NEXT; i; clarify; unfold Cop.sem_binary_operation, Cop.sem_div; unfold Cop.sem_binarith;
+        try solve [eapplyf NEXT; i; clarify; unfold Cop.sem_binary_operation, Cop.sem_div; unfold Cop.sem_binarith;
                   try (erewrite H by et); try (erewrite H0 by et); try (erewrite H1 by et); try (erewrite H2 by et); ss].
       eapply step_sem_cast; et. i. destruct optv; try sim_red;
-        try solve [eapply NEXT; i; clarify; unfold Cop.sem_binary_operation, Cop.sem_div; unfold Cop.sem_binarith;
+        try solve [eapplyf NEXT; i; clarify; unfold Cop.sem_binary_operation, Cop.sem_div; unfold Cop.sem_binarith;
                   try (erewrite H by et); try (erewrite H0 by et); try (erewrite H1 by et); try (erewrite H2 by et); ss].
       des_ifs; sim_red; 
-        eapply NEXT; i; clarify; unfold Cop.sem_binary_operation, Cop.sem_div; unfold Cop.sem_binarith; 
+        eapplyf NEXT; i; clarify; unfold Cop.sem_binary_operation, Cop.sem_div; unfold Cop.sem_binarith; 
           rewrite Heq in *; try (erewrite H by et); try (erewrite H0 by et); try (erewrite H1 by et); try (erewrite H2 by et); ss;
             rewrite Heq0; ss.
     - unfold sem_binarith_c. sim_red. eapply step_sem_cast; et. i. destruct optv; sim_red;
-        try solve [eapply NEXT; i; clarify; unfold Cop.sem_binary_operation, Cop.sem_mod; unfold Cop.sem_binarith;
+        try solve [eapplyf NEXT; i; clarify; unfold Cop.sem_binary_operation, Cop.sem_mod; unfold Cop.sem_binarith;
                   try (erewrite H by et); try (erewrite H0 by et); try (erewrite H1 by et); try (erewrite H2 by et); ss].
       eapply step_sem_cast; et. i. destruct optv; try sim_red;
-        try solve [eapply NEXT; i; clarify; unfold Cop.sem_binary_operation, Cop.sem_mod; unfold Cop.sem_binarith;
+        try solve [eapplyf NEXT; i; clarify; unfold Cop.sem_binary_operation, Cop.sem_mod; unfold Cop.sem_binarith;
                   try (erewrite H by et); try (erewrite H0 by et); try (erewrite H1 by et); try (erewrite H2 by et); ss].
       des_ifs; sim_red; 
-        eapply NEXT; i; clarify; unfold Cop.sem_binary_operation, Cop.sem_mod; unfold Cop.sem_binarith; 
+        eapplyf NEXT; i; clarify; unfold Cop.sem_binary_operation, Cop.sem_mod; unfold Cop.sem_binarith; 
           rewrite Heq in *; try (erewrite H by et); try (erewrite H0 by et); try (erewrite H1 by et); try (erewrite H2 by et); ss;
             rewrite Heq0; ss.
     - unfold sem_binarith_c. sim_red. eapply step_sem_cast; et. i. destruct optv; sim_red;
-        try solve [eapply NEXT; i; clarify; unfold Cop.sem_binary_operation, Cop.sem_and; unfold Cop.sem_binarith;
+        try solve [eapplyf NEXT; i; clarify; unfold Cop.sem_binary_operation, Cop.sem_and; unfold Cop.sem_binarith;
                   try (erewrite H by et); try (erewrite H0 by et); try (erewrite H1 by et); try (erewrite H2 by et); ss].
       eapply step_sem_cast; et. i. destruct optv; try sim_red;
-        try solve [eapply NEXT; i; clarify; unfold Cop.sem_binary_operation, Cop.sem_and; unfold Cop.sem_binarith;
+        try solve [eapplyf NEXT; i; clarify; unfold Cop.sem_binary_operation, Cop.sem_and; unfold Cop.sem_binarith;
                   try (erewrite H by et); try (erewrite H0 by et); try (erewrite H1 by et); try (erewrite H2 by et); ss].
       des_ifs; sim_red; 
-        eapply NEXT; i; clarify; unfold Cop.sem_binary_operation, Cop.sem_and; unfold Cop.sem_binarith; 
+        eapplyf NEXT; i; clarify; unfold Cop.sem_binary_operation, Cop.sem_and; unfold Cop.sem_binarith; 
           rewrite Heq in *; try (erewrite H by et); try (erewrite H0 by et); try (erewrite H1 by et); try (erewrite H2 by et); ss;
             rewrite Heq0; ss.
     - unfold sem_binarith_c. sim_red. eapply step_sem_cast; et. i. destruct optv; sim_red;
-        try solve [eapply NEXT; i; clarify; unfold Cop.sem_binary_operation, Cop.sem_or; unfold Cop.sem_binarith;
+        try solve [eapplyf NEXT; i; clarify; unfold Cop.sem_binary_operation, Cop.sem_or; unfold Cop.sem_binarith;
                   try (erewrite H by et); try (erewrite H0 by et); try (erewrite H1 by et); try (erewrite H2 by et); ss].
       eapply step_sem_cast; et. i. destruct optv; try sim_red;
-        try solve [eapply NEXT; i; clarify; unfold Cop.sem_binary_operation, Cop.sem_or; unfold Cop.sem_binarith;
+        try solve [eapplyf NEXT; i; clarify; unfold Cop.sem_binary_operation, Cop.sem_or; unfold Cop.sem_binarith;
                   try (erewrite H by et); try (erewrite H0 by et); try (erewrite H1 by et); try (erewrite H2 by et); ss].
       des_ifs; sim_red; 
-        eapply NEXT; i; clarify; unfold Cop.sem_binary_operation, Cop.sem_or; unfold Cop.sem_binarith; 
+        eapplyf NEXT; i; clarify; unfold Cop.sem_binary_operation, Cop.sem_or; unfold Cop.sem_binarith; 
           rewrite Heq in *; try (erewrite H by et); try (erewrite H0 by et); try (erewrite H1 by et); try (erewrite H2 by et); ss;
             rewrite Heq0; ss.
     - unfold sem_binarith_c. sim_red. eapply step_sem_cast; et. i. destruct optv; sim_red;
-        try solve [eapply NEXT; i; clarify; unfold Cop.sem_binary_operation, Cop.sem_xor; unfold Cop.sem_binarith;
+        try solve [eapplyf NEXT; i; clarify; unfold Cop.sem_binary_operation, Cop.sem_xor; unfold Cop.sem_binarith;
                   try (erewrite H by et); try (erewrite H0 by et); try (erewrite H1 by et); try (erewrite H2 by et); ss].
       eapply step_sem_cast; et. i. destruct optv; try sim_red;
-        try solve [eapply NEXT; i; clarify; unfold Cop.sem_binary_operation, Cop.sem_xor; unfold Cop.sem_binarith;
+        try solve [eapplyf NEXT; i; clarify; unfold Cop.sem_binary_operation, Cop.sem_xor; unfold Cop.sem_binarith;
                   try (erewrite H by et); try (erewrite H0 by et); try (erewrite H1 by et); try (erewrite H2 by et); ss].
       des_ifs; sim_red; 
-        eapply NEXT; i; clarify; unfold Cop.sem_binary_operation, Cop.sem_xor; unfold Cop.sem_binarith; 
+        eapplyf NEXT; i; clarify; unfold Cop.sem_binary_operation, Cop.sem_xor; unfold Cop.sem_binarith; 
           rewrite Heq in *; try (erewrite H by et); try (erewrite H0 by et); try (erewrite H1 by et); try (erewrite H2 by et); ss;
             rewrite Heq0; ss.
-    - eapply NEXT; i; clarify; unfold Cop.sem_binary_operation, Cop.sem_shl; unfold Cop.sem_binarith; 
+    - eapplyf NEXT; i; clarify; unfold Cop.sem_binary_operation, Cop.sem_shl; unfold Cop.sem_binarith; 
         unfold Cop.sem_shift in *; des_ifs; ss; clarify.
-    - eapply NEXT; i; clarify; unfold Cop.sem_binary_operation, Cop.sem_shr; unfold Cop.sem_binarith; 
+    - eapplyf NEXT; i; clarify; unfold Cop.sem_binary_operation, Cop.sem_shr; unfold Cop.sem_binarith; 
         unfold Cop.sem_shift in *; des_ifs; ss; clarify.
     - des_ifs; unfold cmp_ptr_c; try sim_red; des_ifs_safe; 
-        try solve [unfold cmplu_bool_c; des_ifs; try sim_red; try eapply NEXT; i; ss; clarify; 
+        try solve [unfold cmplu_bool_c; des_ifs; try sim_red; try eapplyf NEXT; i; ss; clarify; 
                     unfold Cop.sem_cmp; rewrite Heq; unfold Cop.cmp_ptr; des_ifs_safe].
       + unfold cmplu_bool_c; des_ifs; try sim_red;
-          try solve [eapply NEXT; i; ss; clarify; unfold Cop.sem_cmp; rewrite Heq; unfold Cop.cmp_ptr; des_ifs_safe].
-          2,3: eapply step_weak_valid_pointer; et; i; des_ifs; sim_red; eapply NEXT; i; ss; clarify;
+          try solve [eapplyf NEXT; i; ss; clarify; unfold Cop.sem_cmp; rewrite Heq; unfold Cop.cmp_ptr; des_ifs_safe].
+          2,3: eapply step_weak_valid_pointer; et; i; des_ifs; sim_red; eapplyf NEXT; i; ss; clarify;
                 unfold Cop.sem_cmp; rewrite Heq; unfold Cop.cmp_ptr; ss; des_ifs_safe; 
                   unfold Mem.weak_valid_pointer in *; clarify.
-        * eapply NEXT; i; ss; clarify. unfold Cop.sem_cmp. rewrite Heq. unfold Cop.cmp_ptr. des_ifs_safe. ss.
+        * eapplyf NEXT; i; ss; clarify. unfold Cop.sem_cmp. rewrite Heq. unfold Cop.cmp_ptr. des_ifs_safe. ss.
           unfold Val.of_bool. des_ifs.
         * eapply step_weak_valid_pointer; et. i. sim_red. eapply step_weak_valid_pointer; et. i.
-          des_ifs; sim_red; eapply NEXT; i; ss; clarify;
+          des_ifs; sim_red; eapplyf NEXT; i; ss; clarify;
           unfold Cop.sem_cmp; rewrite Heq; unfold Cop.cmp_ptr; ss; des_ifs_safe; unfold Mem.weak_valid_pointer in *; clarify;
           unfold Val.of_bool; des_ifs. 
         * unfold ccallU. sim_red. ss. repeat (sim_tau; sim_red). unfold valid_pointerF. sim_red.
@@ -628,42 +632,42 @@ Section PROOF.
           unfold valid_pointerF. sim_red.
           repeat (sim_tau; sim_red). rewrite PSTATE. sim_red. repeat (sim_tau; sim_red).
           repeat match goal with | |- context [Mem.perm_dec ?x ?y ?z ?w ?a] => destruct (Mem.perm_dec x y z w a) end; sim_red;
-            eapply NEXT; i; ss; clarify;
+            eapplyf NEXT; i; ss; clarify;
               unfold Cop.sem_cmp; rewrite Heq; unfold Cop.cmp_ptr; ss; unfold Mem.valid_pointer in *;
                 destruct (eq_block _); des_ifs_safe;
           try solve [eapply map_blk_inj in e0; et; try contradiction];
           try solve [repeat (destruct (Mem.perm_dec _) in Heq3); inv MM; unfold Mem.perm in *; ss;
                       rewrite <- MEM_PERM in *; try contradiction].
       + unfold cmplu_bool_c; des_ifs; try sim_red;
-          try solve [eapply NEXT; i; ss; clarify; unfold Cop.sem_cmp; rewrite Heq; unfold Cop.cmp_ptr; des_ifs_safe].
-          2: eapply step_weak_valid_pointer; et; i; des_ifs; sim_red; eapply NEXT; i; ss; clarify;
+          try solve [eapplyf NEXT; i; ss; clarify; unfold Cop.sem_cmp; rewrite Heq; unfold Cop.cmp_ptr; des_ifs_safe].
+          2: eapply step_weak_valid_pointer; et; i; des_ifs; sim_red; eapplyf NEXT; i; ss; clarify;
                 unfold Cop.sem_cmp; rewrite Heq; unfold Cop.cmp_ptr; ss; des_ifs_safe; 
                   unfold Mem.weak_valid_pointer in *; clarify.
-          eapply NEXT; i; ss; clarify;
+          eapplyf NEXT; i; ss; clarify;
             unfold Cop.sem_cmp; rewrite Heq; unfold Cop.cmp_ptr; ss; unfold Mem.valid_pointer in *; des_ifs_safe.
           unfold Val.of_bool; ss. des_ifs.
       + unfold cmplu_bool_c; des_ifs; try sim_red;
-          try solve [eapply NEXT; i; ss; clarify; unfold Cop.sem_cmp; rewrite Heq; unfold Cop.cmp_ptr; des_ifs_safe].
-          1: eapply NEXT; i; ss; clarify; unfold Cop.sem_cmp; rewrite Heq; unfold Cop.cmp_ptr; des_ifs_safe.
-          2: eapply step_weak_valid_pointer; et; i; des_ifs; sim_red; eapply NEXT; i; ss; clarify;
+          try solve [eapplyf NEXT; i; ss; clarify; unfold Cop.sem_cmp; rewrite Heq; unfold Cop.cmp_ptr; des_ifs_safe].
+          1: eapplyf NEXT; i; ss; clarify; unfold Cop.sem_cmp; rewrite Heq; unfold Cop.cmp_ptr; des_ifs_safe.
+          2: eapply step_weak_valid_pointer; et; i; des_ifs; sim_red; eapplyf NEXT; i; ss; clarify;
                 unfold Cop.sem_cmp; rewrite Heq; unfold Cop.cmp_ptr; ss; des_ifs_safe; 
                   unfold Mem.weak_valid_pointer in *; clarify.
           all: unfold Val.of_bool; unfold Val.cmplu_bool; des_ifs; unfold Int64.cmpu; rewrite Heq1; ss.
       + unfold cmplu_bool_c; des_ifs; try sim_red;
-          try solve [eapply NEXT; i; ss; clarify; unfold Cop.sem_cmp; rewrite Heq; unfold Cop.cmp_ptr; des_ifs_safe].
-          2: eapply step_weak_valid_pointer; et; i; des_ifs; sim_red; eapply NEXT; i; ss; clarify;
+          try solve [eapplyf NEXT; i; ss; clarify; unfold Cop.sem_cmp; rewrite Heq; unfold Cop.cmp_ptr; des_ifs_safe].
+          2: eapply step_weak_valid_pointer; et; i; des_ifs; sim_red; eapplyf NEXT; i; ss; clarify;
                 unfold Cop.sem_cmp; rewrite Heq; unfold Cop.cmp_ptr; ss; des_ifs_safe; 
                   unfold Mem.weak_valid_pointer in *; clarify.
-          eapply NEXT; i; ss; clarify;
+          eapplyf NEXT; i; ss; clarify;
             unfold Cop.sem_cmp; rewrite Heq; unfold Cop.cmp_ptr; ss; unfold Mem.valid_pointer in *; des_ifs_safe.
           unfold Val.of_bool; ss. des_ifs.
       + unfold cmplu_bool_c; des_ifs; try sim_red;
-          try solve [eapply NEXT; i; ss; clarify; unfold Cop.sem_cmp; rewrite Heq; unfold Cop.cmp_ptr; des_ifs_safe].
-        * eapply step_weak_valid_pointer; et; i; des_ifs; sim_red; eapply NEXT; i; ss; clarify;
+          try solve [eapplyf NEXT; i; ss; clarify; unfold Cop.sem_cmp; rewrite Heq; unfold Cop.cmp_ptr; des_ifs_safe].
+        * eapply step_weak_valid_pointer; et; i; des_ifs; sim_red; eapplyf NEXT; i; ss; clarify;
                 unfold Cop.sem_cmp; rewrite Heq; unfold Cop.cmp_ptr; ss; des_ifs_safe; 
                   unfold Mem.weak_valid_pointer in *; clarify.
         * eapply step_weak_valid_pointer; et. i. sim_red. eapply step_weak_valid_pointer; et. i.
-          des_ifs; sim_red; eapply NEXT; i; ss; clarify;
+          des_ifs; sim_red; eapplyf NEXT; i; ss; clarify;
           unfold Cop.sem_cmp; rewrite Heq; unfold Cop.cmp_ptr; ss; des_ifs_safe; unfold Mem.weak_valid_pointer in *; clarify;
           unfold Val.of_bool; des_ifs. 
         * unfold ccallU. sim_red. ss. repeat (sim_tau; sim_red). unfold valid_pointerF. sim_red.
@@ -671,26 +675,26 @@ Section PROOF.
           unfold valid_pointerF. sim_red.
           repeat (sim_tau; sim_red). rewrite PSTATE. sim_red. repeat (sim_tau; sim_red).
           repeat match goal with | |- context [Mem.perm_dec ?x ?y ?z ?w ?a] => destruct (Mem.perm_dec x y z w a) end; sim_red;
-            eapply NEXT; i; ss; clarify;
+            eapplyf NEXT; i; ss; clarify;
               unfold Cop.sem_cmp; rewrite Heq; unfold Cop.cmp_ptr; ss; unfold Mem.valid_pointer in *;
                 destruct (eq_block _); des_ifs_safe;
           try solve [eapply map_blk_inj in e0; et; try contradiction];
           try solve [repeat (destruct (Mem.perm_dec _) in Heq3); inv MM; unfold Mem.perm in *; ss;
                       rewrite <- MEM_PERM in *; try contradiction].
       + unfold cmplu_bool_c; des_ifs; try sim_red;
-          try solve [eapply NEXT; i; ss; clarify; unfold Cop.sem_cmp; rewrite Heq; unfold Cop.cmp_ptr; des_ifs_safe].
-          1: eapply NEXT; i; ss; clarify; unfold Cop.sem_cmp; rewrite Heq; unfold Cop.cmp_ptr; des_ifs_safe.
-          2: eapply step_weak_valid_pointer; et; i; des_ifs; sim_red; eapply NEXT; i; ss; clarify;
+          try solve [eapplyf NEXT; i; ss; clarify; unfold Cop.sem_cmp; rewrite Heq; unfold Cop.cmp_ptr; des_ifs_safe].
+          1: eapplyf NEXT; i; ss; clarify; unfold Cop.sem_cmp; rewrite Heq; unfold Cop.cmp_ptr; des_ifs_safe.
+          2: eapply step_weak_valid_pointer; et; i; des_ifs; sim_red; eapplyf NEXT; i; ss; clarify;
                 unfold Cop.sem_cmp; rewrite Heq; unfold Cop.cmp_ptr; ss; des_ifs_safe; 
                   unfold Mem.weak_valid_pointer in *; clarify.
           all: unfold Val.of_bool; unfold Val.cmplu_bool; des_ifs; unfold Int64.cmpu; rewrite Heq1; ss.
       + unfold cmplu_bool_c; des_ifs; try sim_red;
-          try solve [eapply NEXT; i; ss; clarify; unfold Cop.sem_cmp; rewrite Heq; unfold Cop.cmp_ptr; des_ifs_safe].
-        * eapply step_weak_valid_pointer; et; i; des_ifs; sim_red; eapply NEXT; i; ss; clarify;
+          try solve [eapplyf NEXT; i; ss; clarify; unfold Cop.sem_cmp; rewrite Heq; unfold Cop.cmp_ptr; des_ifs_safe].
+        * eapply step_weak_valid_pointer; et; i; des_ifs; sim_red; eapplyf NEXT; i; ss; clarify;
                 unfold Cop.sem_cmp; rewrite Heq; unfold Cop.cmp_ptr; ss; des_ifs_safe; 
                   unfold Mem.weak_valid_pointer in *; clarify.
         * eapply step_weak_valid_pointer; et. i. sim_red. eapply step_weak_valid_pointer; et. i.
-          des_ifs; sim_red; eapply NEXT; i; ss; clarify;
+          des_ifs; sim_red; eapplyf NEXT; i; ss; clarify;
           unfold Cop.sem_cmp; rewrite Heq; unfold Cop.cmp_ptr; ss; des_ifs_safe; unfold Mem.weak_valid_pointer in *; clarify;
           unfold Val.of_bool; des_ifs. 
         * unfold ccallU. sim_red. ss. repeat (sim_tau; sim_red). unfold valid_pointerF. sim_red.
@@ -698,35 +702,35 @@ Section PROOF.
           unfold valid_pointerF. sim_red.
           repeat (sim_tau; sim_red). rewrite PSTATE. sim_red. repeat (sim_tau; sim_red).
           repeat match goal with | |- context [Mem.perm_dec ?x ?y ?z ?w ?a] => destruct (Mem.perm_dec x y z w a) end; sim_red;
-            eapply NEXT; i; ss; clarify;
+            eapplyf NEXT; i; ss; clarify;
               unfold Cop.sem_cmp; rewrite Heq; unfold Cop.cmp_ptr; ss; unfold Mem.valid_pointer in *;
                 destruct (eq_block _); des_ifs_safe;
           try solve [eapply map_blk_inj in e0; et; try contradiction];
           try solve [repeat (destruct (Mem.perm_dec _) in Heq3); inv MM; unfold Mem.perm in *; ss;
                       rewrite <- MEM_PERM in *; try contradiction].
     + unfold sem_binarith_c. sim_red. eapply step_sem_cast; et. i. destruct optv; sim_red;
-        try solve [ eapply NEXT; i; clarify; unfold Cop.sem_binary_operation, Cop.sem_cmp; unfold Cop.sem_binarith; rewrite Heq;
+        try solve [ eapplyf NEXT; i; clarify; unfold Cop.sem_binary_operation, Cop.sem_cmp; unfold Cop.sem_binarith; rewrite Heq;
                   try (erewrite H by et); try (erewrite H0 by et); try (erewrite H1 by et); try (erewrite H2 by et); ss].
       eapply step_sem_cast; et. i. destruct optv; try sim_red;
-        try solve [eapply NEXT; i; clarify; unfold Cop.sem_binary_operation, Cop.sem_cmp; unfold Cop.sem_binarith; rewrite Heq;
+        try solve [eapplyf NEXT; i; clarify; unfold Cop.sem_binary_operation, Cop.sem_cmp; unfold Cop.sem_binarith; rewrite Heq;
                   try (erewrite H by et); try (erewrite H0 by et); try (erewrite H1 by et); try (erewrite H2 by et); ss].
       des_ifs; sim_red; 
-        eapply NEXT; i; clarify; unfold Cop.sem_binary_operation, Cop.sem_cmp; unfold Cop.sem_binarith; 
+        eapplyf NEXT; i; clarify; unfold Cop.sem_binary_operation, Cop.sem_cmp; unfold Cop.sem_binarith; 
           rewrite Heq in *; rewrite Heq0 in *;
             try (erewrite H by et); try (erewrite H0 by et); try (erewrite H1 by et); try (erewrite H2 by et); ss.
       all: unfold Val.of_bool; unfold Val.cmplu_bool; des_ifs; unfold Int64.cmpu; rewrite Heq1; ss.
     - des_ifs; unfold cmp_ptr_c; try sim_red; des_ifs_safe; 
-        try solve [unfold cmplu_bool_c; des_ifs; try sim_red; try eapply NEXT; i; ss; clarify; 
+        try solve [unfold cmplu_bool_c; des_ifs; try sim_red; try eapplyf NEXT; i; ss; clarify; 
                     unfold Cop.sem_cmp; rewrite Heq; unfold Cop.cmp_ptr; des_ifs_safe].
       + unfold cmplu_bool_c; des_ifs; try sim_red;
-          try solve [eapply NEXT; i; ss; clarify; unfold Cop.sem_cmp; rewrite Heq; unfold Cop.cmp_ptr; des_ifs_safe].
-          2,3: eapply step_weak_valid_pointer; et; i; des_ifs; sim_red; eapply NEXT; i; ss; clarify;
+          try solve [eapplyf NEXT; i; ss; clarify; unfold Cop.sem_cmp; rewrite Heq; unfold Cop.cmp_ptr; des_ifs_safe].
+          2,3: eapply step_weak_valid_pointer; et; i; des_ifs; sim_red; eapplyf NEXT; i; ss; clarify;
                 unfold Cop.sem_cmp; rewrite Heq; unfold Cop.cmp_ptr; ss; des_ifs_safe; 
                   unfold Mem.weak_valid_pointer in *; clarify.
-        * eapply NEXT; i; ss; clarify. unfold Cop.sem_cmp. rewrite Heq. unfold Cop.cmp_ptr. des_ifs_safe. ss.
+        * eapplyf NEXT; i; ss; clarify. unfold Cop.sem_cmp. rewrite Heq. unfold Cop.cmp_ptr. des_ifs_safe. ss.
           unfold Val.of_bool. des_ifs.
         * eapply step_weak_valid_pointer; et. i. sim_red. eapply step_weak_valid_pointer; et. i.
-          des_ifs; sim_red; eapply NEXT; i; ss; clarify;
+          des_ifs; sim_red; eapplyf NEXT; i; ss; clarify;
           unfold Cop.sem_cmp; rewrite Heq; unfold Cop.cmp_ptr; ss; des_ifs_safe; unfold Mem.weak_valid_pointer in *; clarify;
           unfold Val.of_bool; des_ifs. 
         * unfold ccallU. sim_red. ss. repeat (sim_tau; sim_red). unfold valid_pointerF. sim_red.
@@ -734,42 +738,42 @@ Section PROOF.
           unfold valid_pointerF. sim_red.
           repeat (sim_tau; sim_red). rewrite PSTATE. sim_red. repeat (sim_tau; sim_red).
           repeat match goal with | |- context [Mem.perm_dec ?x ?y ?z ?w ?a] => destruct (Mem.perm_dec x y z w a) end; sim_red;
-            eapply NEXT; i; ss; clarify;
+            eapplyf NEXT; i; ss; clarify;
               unfold Cop.sem_cmp; rewrite Heq; unfold Cop.cmp_ptr; ss; unfold Mem.valid_pointer in *;
                 destruct (eq_block _); des_ifs_safe;
           try solve [eapply map_blk_inj in e0; et; try contradiction];
           try solve [repeat (destruct (Mem.perm_dec _) in Heq3); inv MM; unfold Mem.perm in *; ss;
                       rewrite <- MEM_PERM in *; try contradiction].
       + unfold cmplu_bool_c; des_ifs; try sim_red;
-          try solve [eapply NEXT; i; ss; clarify; unfold Cop.sem_cmp; rewrite Heq; unfold Cop.cmp_ptr; des_ifs_safe].
-          2: eapply step_weak_valid_pointer; et; i; des_ifs; sim_red; eapply NEXT; i; ss; clarify;
+          try solve [eapplyf NEXT; i; ss; clarify; unfold Cop.sem_cmp; rewrite Heq; unfold Cop.cmp_ptr; des_ifs_safe].
+          2: eapply step_weak_valid_pointer; et; i; des_ifs; sim_red; eapplyf NEXT; i; ss; clarify;
                 unfold Cop.sem_cmp; rewrite Heq; unfold Cop.cmp_ptr; ss; des_ifs_safe; 
                   unfold Mem.weak_valid_pointer in *; clarify.
-          eapply NEXT; i; ss; clarify;
+          eapplyf NEXT; i; ss; clarify;
             unfold Cop.sem_cmp; rewrite Heq; unfold Cop.cmp_ptr; ss; unfold Mem.valid_pointer in *; des_ifs_safe.
           unfold Val.of_bool; ss. des_ifs.
       + unfold cmplu_bool_c; des_ifs; try sim_red;
-          try solve [eapply NEXT; i; ss; clarify; unfold Cop.sem_cmp; rewrite Heq; unfold Cop.cmp_ptr; des_ifs_safe].
-          1: eapply NEXT; i; ss; clarify; unfold Cop.sem_cmp; rewrite Heq; unfold Cop.cmp_ptr; des_ifs_safe.
-          2: eapply step_weak_valid_pointer; et; i; des_ifs; sim_red; eapply NEXT; i; ss; clarify;
+          try solve [eapplyf NEXT; i; ss; clarify; unfold Cop.sem_cmp; rewrite Heq; unfold Cop.cmp_ptr; des_ifs_safe].
+          1: eapplyf NEXT; i; ss; clarify; unfold Cop.sem_cmp; rewrite Heq; unfold Cop.cmp_ptr; des_ifs_safe.
+          2: eapply step_weak_valid_pointer; et; i; des_ifs; sim_red; eapplyf NEXT; i; ss; clarify;
                 unfold Cop.sem_cmp; rewrite Heq; unfold Cop.cmp_ptr; ss; des_ifs_safe; 
                   unfold Mem.weak_valid_pointer in *; clarify.
           all: unfold Val.of_bool; unfold Val.cmplu_bool; des_ifs; unfold Int64.cmpu; rewrite Heq1; ss.
       + unfold cmplu_bool_c; des_ifs; try sim_red;
-          try solve [eapply NEXT; i; ss; clarify; unfold Cop.sem_cmp; rewrite Heq; unfold Cop.cmp_ptr; des_ifs_safe].
-          2: eapply step_weak_valid_pointer; et; i; des_ifs; sim_red; eapply NEXT; i; ss; clarify;
+          try solve [eapplyf NEXT; i; ss; clarify; unfold Cop.sem_cmp; rewrite Heq; unfold Cop.cmp_ptr; des_ifs_safe].
+          2: eapply step_weak_valid_pointer; et; i; des_ifs; sim_red; eapplyf NEXT; i; ss; clarify;
                 unfold Cop.sem_cmp; rewrite Heq; unfold Cop.cmp_ptr; ss; des_ifs_safe; 
                   unfold Mem.weak_valid_pointer in *; clarify.
-          eapply NEXT; i; ss; clarify;
+          eapplyf NEXT; i; ss; clarify;
             unfold Cop.sem_cmp; rewrite Heq; unfold Cop.cmp_ptr; ss; unfold Mem.valid_pointer in *; des_ifs_safe.
           unfold Val.of_bool; ss. des_ifs.
       + unfold cmplu_bool_c; des_ifs; try sim_red;
-          try solve [eapply NEXT; i; ss; clarify; unfold Cop.sem_cmp; rewrite Heq; unfold Cop.cmp_ptr; des_ifs_safe].
-        * eapply step_weak_valid_pointer; et; i; des_ifs; sim_red; eapply NEXT; i; ss; clarify;
+          try solve [eapplyf NEXT; i; ss; clarify; unfold Cop.sem_cmp; rewrite Heq; unfold Cop.cmp_ptr; des_ifs_safe].
+        * eapply step_weak_valid_pointer; et; i; des_ifs; sim_red; eapplyf NEXT; i; ss; clarify;
                 unfold Cop.sem_cmp; rewrite Heq; unfold Cop.cmp_ptr; ss; des_ifs_safe; 
                   unfold Mem.weak_valid_pointer in *; clarify.
         * eapply step_weak_valid_pointer; et. i. sim_red. eapply step_weak_valid_pointer; et. i.
-          des_ifs; sim_red; eapply NEXT; i; ss; clarify;
+          des_ifs; sim_red; eapplyf NEXT; i; ss; clarify;
           unfold Cop.sem_cmp; rewrite Heq; unfold Cop.cmp_ptr; ss; des_ifs_safe; unfold Mem.weak_valid_pointer in *; clarify;
           unfold Val.of_bool; des_ifs. 
         * unfold ccallU. sim_red. ss. repeat (sim_tau; sim_red). unfold valid_pointerF. sim_red.
@@ -777,26 +781,26 @@ Section PROOF.
           unfold valid_pointerF. sim_red.
           repeat (sim_tau; sim_red). rewrite PSTATE. sim_red. repeat (sim_tau; sim_red).
           repeat match goal with | |- context [Mem.perm_dec ?x ?y ?z ?w ?a] => destruct (Mem.perm_dec x y z w a) end; sim_red;
-            eapply NEXT; i; ss; clarify;
+            eapplyf NEXT; i; ss; clarify;
               unfold Cop.sem_cmp; rewrite Heq; unfold Cop.cmp_ptr; ss; unfold Mem.valid_pointer in *;
                 destruct (eq_block _); des_ifs_safe;
           try solve [eapply map_blk_inj in e0; et; try contradiction];
           try solve [repeat (destruct (Mem.perm_dec _) in Heq3); inv MM; unfold Mem.perm in *; ss;
                       rewrite <- MEM_PERM in *; try contradiction].
       + unfold cmplu_bool_c; des_ifs; try sim_red;
-          try solve [eapply NEXT; i; ss; clarify; unfold Cop.sem_cmp; rewrite Heq; unfold Cop.cmp_ptr; des_ifs_safe].
-          1: eapply NEXT; i; ss; clarify; unfold Cop.sem_cmp; rewrite Heq; unfold Cop.cmp_ptr; des_ifs_safe.
-          2: eapply step_weak_valid_pointer; et; i; des_ifs; sim_red; eapply NEXT; i; ss; clarify;
+          try solve [eapplyf NEXT; i; ss; clarify; unfold Cop.sem_cmp; rewrite Heq; unfold Cop.cmp_ptr; des_ifs_safe].
+          1: eapplyf NEXT; i; ss; clarify; unfold Cop.sem_cmp; rewrite Heq; unfold Cop.cmp_ptr; des_ifs_safe.
+          2: eapply step_weak_valid_pointer; et; i; des_ifs; sim_red; eapplyf NEXT; i; ss; clarify;
                 unfold Cop.sem_cmp; rewrite Heq; unfold Cop.cmp_ptr; ss; des_ifs_safe; 
                   unfold Mem.weak_valid_pointer in *; clarify.
           all: unfold Val.of_bool; unfold Val.cmplu_bool; des_ifs; unfold Int64.cmpu; rewrite Heq1; ss.
       + unfold cmplu_bool_c; des_ifs; try sim_red;
-          try solve [eapply NEXT; i; ss; clarify; unfold Cop.sem_cmp; rewrite Heq; unfold Cop.cmp_ptr; des_ifs_safe].
-        * eapply step_weak_valid_pointer; et; i; des_ifs; sim_red; eapply NEXT; i; ss; clarify;
+          try solve [eapplyf NEXT; i; ss; clarify; unfold Cop.sem_cmp; rewrite Heq; unfold Cop.cmp_ptr; des_ifs_safe].
+        * eapply step_weak_valid_pointer; et; i; des_ifs; sim_red; eapplyf NEXT; i; ss; clarify;
                 unfold Cop.sem_cmp; rewrite Heq; unfold Cop.cmp_ptr; ss; des_ifs_safe; 
                   unfold Mem.weak_valid_pointer in *; clarify.
         * eapply step_weak_valid_pointer; et. i. sim_red. eapply step_weak_valid_pointer; et. i.
-          des_ifs; sim_red; eapply NEXT; i; ss; clarify;
+          des_ifs; sim_red; eapplyf NEXT; i; ss; clarify;
           unfold Cop.sem_cmp; rewrite Heq; unfold Cop.cmp_ptr; ss; des_ifs_safe; unfold Mem.weak_valid_pointer in *; clarify;
           unfold Val.of_bool; des_ifs. 
         * unfold ccallU. sim_red. ss. repeat (sim_tau; sim_red). unfold valid_pointerF. sim_red.
@@ -804,35 +808,35 @@ Section PROOF.
           unfold valid_pointerF. sim_red.
           repeat (sim_tau; sim_red). rewrite PSTATE. sim_red. repeat (sim_tau; sim_red).
           repeat match goal with | |- context [Mem.perm_dec ?x ?y ?z ?w ?a] => destruct (Mem.perm_dec x y z w a) end; sim_red;
-            eapply NEXT; i; ss; clarify;
+            eapplyf NEXT; i; ss; clarify;
               unfold Cop.sem_cmp; rewrite Heq; unfold Cop.cmp_ptr; ss; unfold Mem.valid_pointer in *;
                 destruct (eq_block _); des_ifs_safe;
           try solve [eapply map_blk_inj in e0; et; try contradiction];
           try solve [repeat (destruct (Mem.perm_dec _) in Heq3); inv MM; unfold Mem.perm in *; ss;
                       rewrite <- MEM_PERM in *; try contradiction].
     + unfold sem_binarith_c. sim_red. eapply step_sem_cast; et. i. destruct optv; sim_red;
-        try solve [ eapply NEXT; i; clarify; unfold Cop.sem_binary_operation, Cop.sem_cmp; unfold Cop.sem_binarith; rewrite Heq;
+        try solve [ eapplyf NEXT; i; clarify; unfold Cop.sem_binary_operation, Cop.sem_cmp; unfold Cop.sem_binarith; rewrite Heq;
                   try (erewrite H by et); try (erewrite H0 by et); try (erewrite H1 by et); try (erewrite H2 by et); ss].
       eapply step_sem_cast; et. i. destruct optv; try sim_red;
-        try solve [eapply NEXT; i; clarify; unfold Cop.sem_binary_operation, Cop.sem_cmp; unfold Cop.sem_binarith; rewrite Heq;
+        try solve [eapplyf NEXT; i; clarify; unfold Cop.sem_binary_operation, Cop.sem_cmp; unfold Cop.sem_binarith; rewrite Heq;
                   try (erewrite H by et); try (erewrite H0 by et); try (erewrite H1 by et); try (erewrite H2 by et); ss].
       des_ifs; sim_red; 
-        eapply NEXT; i; clarify; unfold Cop.sem_binary_operation, Cop.sem_cmp; unfold Cop.sem_binarith; 
+        eapplyf NEXT; i; clarify; unfold Cop.sem_binary_operation, Cop.sem_cmp; unfold Cop.sem_binarith; 
           rewrite Heq in *; rewrite Heq0 in *;
             try (erewrite H by et); try (erewrite H0 by et); try (erewrite H1 by et); try (erewrite H2 by et); ss.
       all: unfold Val.of_bool; unfold Val.cmplu_bool; des_ifs; unfold Int64.cmpu; rewrite Heq1; ss.
     - des_ifs; unfold cmp_ptr_c; try sim_red; des_ifs_safe; 
-        try solve [unfold cmplu_bool_c; des_ifs; try sim_red; try eapply NEXT; i; ss; clarify; 
+        try solve [unfold cmplu_bool_c; des_ifs; try sim_red; try eapplyf NEXT; i; ss; clarify; 
                     unfold Cop.sem_cmp; rewrite Heq; unfold Cop.cmp_ptr; des_ifs_safe].
       + unfold cmplu_bool_c; des_ifs; try sim_red;
-          try solve [eapply NEXT; i; ss; clarify; unfold Cop.sem_cmp; rewrite Heq; unfold Cop.cmp_ptr; des_ifs_safe].
-          2,3: eapply step_weak_valid_pointer; et; i; des_ifs; sim_red; eapply NEXT; i; ss; clarify;
+          try solve [eapplyf NEXT; i; ss; clarify; unfold Cop.sem_cmp; rewrite Heq; unfold Cop.cmp_ptr; des_ifs_safe].
+          2,3: eapply step_weak_valid_pointer; et; i; des_ifs; sim_red; eapplyf NEXT; i; ss; clarify;
                 unfold Cop.sem_cmp; rewrite Heq; unfold Cop.cmp_ptr; ss; des_ifs_safe; 
                   unfold Mem.weak_valid_pointer in *; clarify.
-        * eapply NEXT; i; ss; clarify. unfold Cop.sem_cmp. rewrite Heq. unfold Cop.cmp_ptr. des_ifs_safe. ss.
+        * eapplyf NEXT; i; ss; clarify. unfold Cop.sem_cmp. rewrite Heq. unfold Cop.cmp_ptr. des_ifs_safe. ss.
           unfold Val.of_bool. des_ifs.
         * eapply step_weak_valid_pointer; et. i. sim_red. eapply step_weak_valid_pointer; et. i.
-          des_ifs; sim_red; eapply NEXT; i; ss; clarify;
+          des_ifs; sim_red; eapplyf NEXT; i; ss; clarify;
           unfold Cop.sem_cmp; rewrite Heq; unfold Cop.cmp_ptr; ss; des_ifs_safe; unfold Mem.weak_valid_pointer in *; clarify;
           unfold Val.of_bool; des_ifs. 
         * unfold ccallU. sim_red. ss. repeat (sim_tau; sim_red). unfold valid_pointerF. sim_red.
@@ -840,41 +844,41 @@ Section PROOF.
           unfold valid_pointerF. sim_red.
           repeat (sim_tau; sim_red). rewrite PSTATE. sim_red. repeat (sim_tau; sim_red).
           repeat match goal with | |- context [Mem.perm_dec ?x ?y ?z ?w ?a] => destruct (Mem.perm_dec x y z w a) end; sim_red;
-            eapply NEXT; i; ss; clarify;
+            eapplyf NEXT; i; ss; clarify;
               unfold Cop.sem_cmp; rewrite Heq; unfold Cop.cmp_ptr; ss; unfold Mem.valid_pointer in *;
                 destruct (eq_block _); des_ifs_safe;
           try solve [eapply map_blk_inj in e0; et; try contradiction];
           repeat (destruct (Mem.perm_dec _)); inv MM; unfold Mem.perm in *; ss.
       + unfold cmplu_bool_c; des_ifs; try sim_red;
-          try solve [eapply NEXT; i; ss; clarify; unfold Cop.sem_cmp; rewrite Heq; unfold Cop.cmp_ptr; des_ifs_safe].
-          2: eapply step_weak_valid_pointer; et; i; des_ifs; sim_red; eapply NEXT; i; ss; clarify;
+          try solve [eapplyf NEXT; i; ss; clarify; unfold Cop.sem_cmp; rewrite Heq; unfold Cop.cmp_ptr; des_ifs_safe].
+          2: eapply step_weak_valid_pointer; et; i; des_ifs; sim_red; eapplyf NEXT; i; ss; clarify;
                 unfold Cop.sem_cmp; rewrite Heq; unfold Cop.cmp_ptr; ss; des_ifs_safe; 
                   unfold Mem.weak_valid_pointer in *; clarify.
-          eapply NEXT; i; ss; clarify;
+          eapplyf NEXT; i; ss; clarify;
             unfold Cop.sem_cmp; rewrite Heq; unfold Cop.cmp_ptr; ss; unfold Mem.valid_pointer in *; des_ifs_safe.
           unfold Val.of_bool; ss. des_ifs.
       + unfold cmplu_bool_c; des_ifs; try sim_red;
-          try solve [eapply NEXT; i; ss; clarify; unfold Cop.sem_cmp; rewrite Heq; unfold Cop.cmp_ptr; des_ifs_safe].
-          1: eapply NEXT; i; ss; clarify; unfold Cop.sem_cmp; rewrite Heq; unfold Cop.cmp_ptr; des_ifs_safe.
-          2: eapply step_weak_valid_pointer; et; i; des_ifs; sim_red; eapply NEXT; i; ss; clarify;
+          try solve [eapplyf NEXT; i; ss; clarify; unfold Cop.sem_cmp; rewrite Heq; unfold Cop.cmp_ptr; des_ifs_safe].
+          1: eapplyf NEXT; i; ss; clarify; unfold Cop.sem_cmp; rewrite Heq; unfold Cop.cmp_ptr; des_ifs_safe.
+          2: eapply step_weak_valid_pointer; et; i; des_ifs; sim_red; eapplyf NEXT; i; ss; clarify;
                 unfold Cop.sem_cmp; rewrite Heq; unfold Cop.cmp_ptr; ss; des_ifs_safe; 
                   unfold Mem.weak_valid_pointer in *; clarify.
           all: unfold Val.of_bool; unfold Val.cmplu_bool; des_ifs; unfold Int64.cmpu; rewrite Heq1; ss.
       + unfold cmplu_bool_c; des_ifs; try sim_red;
-          try solve [eapply NEXT; i; ss; clarify; unfold Cop.sem_cmp; rewrite Heq; unfold Cop.cmp_ptr; des_ifs_safe].
-          2: eapply step_weak_valid_pointer; et; i; des_ifs; sim_red; eapply NEXT; i; ss; clarify;
+          try solve [eapplyf NEXT; i; ss; clarify; unfold Cop.sem_cmp; rewrite Heq; unfold Cop.cmp_ptr; des_ifs_safe].
+          2: eapply step_weak_valid_pointer; et; i; des_ifs; sim_red; eapplyf NEXT; i; ss; clarify;
                 unfold Cop.sem_cmp; rewrite Heq; unfold Cop.cmp_ptr; ss; des_ifs_safe; 
                   unfold Mem.weak_valid_pointer in *; clarify.
-          eapply NEXT; i; ss; clarify;
+          eapplyf NEXT; i; ss; clarify;
             unfold Cop.sem_cmp; rewrite Heq; unfold Cop.cmp_ptr; ss; unfold Mem.valid_pointer in *; des_ifs_safe.
           unfold Val.of_bool; ss. des_ifs.
       + unfold cmplu_bool_c; des_ifs; try sim_red;
-          try solve [eapply NEXT; i; ss; clarify; unfold Cop.sem_cmp; rewrite Heq; unfold Cop.cmp_ptr; des_ifs_safe].
-        * eapply step_weak_valid_pointer; et; i; des_ifs; sim_red; eapply NEXT; i; ss; clarify;
+          try solve [eapplyf NEXT; i; ss; clarify; unfold Cop.sem_cmp; rewrite Heq; unfold Cop.cmp_ptr; des_ifs_safe].
+        * eapply step_weak_valid_pointer; et; i; des_ifs; sim_red; eapplyf NEXT; i; ss; clarify;
                 unfold Cop.sem_cmp; rewrite Heq; unfold Cop.cmp_ptr; ss; des_ifs_safe; 
                   unfold Mem.weak_valid_pointer in *; clarify.
         * eapply step_weak_valid_pointer; et. i. sim_red. eapply step_weak_valid_pointer; et. i.
-          des_ifs; sim_red; eapply NEXT; i; ss; clarify;
+          des_ifs; sim_red; eapplyf NEXT; i; ss; clarify;
           unfold Cop.sem_cmp; rewrite Heq; unfold Cop.cmp_ptr; ss; des_ifs_safe; unfold Mem.weak_valid_pointer in *; clarify;
           unfold Val.of_bool; des_ifs. 
         * unfold ccallU. sim_red. ss. repeat (sim_tau; sim_red). unfold valid_pointerF. sim_red.
@@ -882,25 +886,25 @@ Section PROOF.
           unfold valid_pointerF. sim_red.
           repeat (sim_tau; sim_red). rewrite PSTATE. sim_red. repeat (sim_tau; sim_red).
           repeat match goal with | |- context [Mem.perm_dec ?x ?y ?z ?w ?a] => destruct (Mem.perm_dec x y z w a) end; sim_red;
-            eapply NEXT; i; ss; clarify;
+            eapplyf NEXT; i; ss; clarify;
               unfold Cop.sem_cmp; rewrite Heq; unfold Cop.cmp_ptr; ss; unfold Mem.valid_pointer in *;
                 destruct (eq_block _); des_ifs_safe;
           try solve [eapply map_blk_inj in e0; et; try contradiction];
           repeat (destruct (Mem.perm_dec _)); inv MM; unfold Mem.perm in *; ss.
       + unfold cmplu_bool_c; des_ifs; try sim_red;
-          try solve [eapply NEXT; i; ss; clarify; unfold Cop.sem_cmp; rewrite Heq; unfold Cop.cmp_ptr; des_ifs_safe].
-          1: eapply NEXT; i; ss; clarify; unfold Cop.sem_cmp; rewrite Heq; unfold Cop.cmp_ptr; des_ifs_safe.
-          2: eapply step_weak_valid_pointer; et; i; des_ifs; sim_red; eapply NEXT; i; ss; clarify;
+          try solve [eapplyf NEXT; i; ss; clarify; unfold Cop.sem_cmp; rewrite Heq; unfold Cop.cmp_ptr; des_ifs_safe].
+          1: eapplyf NEXT; i; ss; clarify; unfold Cop.sem_cmp; rewrite Heq; unfold Cop.cmp_ptr; des_ifs_safe.
+          2: eapply step_weak_valid_pointer; et; i; des_ifs; sim_red; eapplyf NEXT; i; ss; clarify;
                 unfold Cop.sem_cmp; rewrite Heq; unfold Cop.cmp_ptr; ss; des_ifs_safe; 
                   unfold Mem.weak_valid_pointer in *; clarify.
           all: unfold Val.of_bool; unfold Val.cmplu_bool; des_ifs; unfold Int64.cmpu; rewrite Heq1; ss.
       + unfold cmplu_bool_c; des_ifs; try sim_red;
-          try solve [eapply NEXT; i; ss; clarify; unfold Cop.sem_cmp; rewrite Heq; unfold Cop.cmp_ptr; des_ifs_safe].
-        * eapply step_weak_valid_pointer; et; i; des_ifs; sim_red; eapply NEXT; i; ss; clarify;
+          try solve [eapplyf NEXT; i; ss; clarify; unfold Cop.sem_cmp; rewrite Heq; unfold Cop.cmp_ptr; des_ifs_safe].
+        * eapply step_weak_valid_pointer; et; i; des_ifs; sim_red; eapplyf NEXT; i; ss; clarify;
                 unfold Cop.sem_cmp; rewrite Heq; unfold Cop.cmp_ptr; ss; des_ifs_safe; 
                   unfold Mem.weak_valid_pointer in *; clarify.
         * eapply step_weak_valid_pointer; et. i. sim_red. eapply step_weak_valid_pointer; et. i.
-          des_ifs; sim_red; eapply NEXT; i; ss; clarify;
+          des_ifs; sim_red; eapplyf NEXT; i; ss; clarify;
           unfold Cop.sem_cmp; rewrite Heq; unfold Cop.cmp_ptr; ss; des_ifs_safe; unfold Mem.weak_valid_pointer in *; clarify;
           unfold Val.of_bool; des_ifs. 
         * unfold ccallU. sim_red. ss. repeat (sim_tau; sim_red). unfold valid_pointerF. sim_red.
@@ -908,34 +912,34 @@ Section PROOF.
           unfold valid_pointerF. sim_red.
           repeat (sim_tau; sim_red). rewrite PSTATE. sim_red. repeat (sim_tau; sim_red).
           repeat match goal with | |- context [Mem.perm_dec ?x ?y ?z ?w ?a] => destruct (Mem.perm_dec x y z w a) end; sim_red;
-            eapply NEXT; i; ss; clarify;
+            eapplyf NEXT; i; ss; clarify;
               unfold Cop.sem_cmp; rewrite Heq; unfold Cop.cmp_ptr; ss; unfold Mem.valid_pointer in *;
                 destruct (eq_block _); des_ifs_safe;
           try solve [eapply map_blk_inj in e0; et; try contradiction];
           repeat (destruct (Mem.perm_dec _)); inv MM; unfold Mem.perm in *; ss.
     + unfold sem_binarith_c. sim_red. eapply step_sem_cast; et. i. destruct optv; sim_red;
-        try solve [ eapply NEXT; i; clarify; unfold Cop.sem_binary_operation, Cop.sem_cmp; unfold Cop.sem_binarith; rewrite Heq;
+        try solve [ eapplyf NEXT; i; clarify; unfold Cop.sem_binary_operation, Cop.sem_cmp; unfold Cop.sem_binarith; rewrite Heq;
                   try (erewrite H by et); try (erewrite H0 by et); try (erewrite H1 by et); try (erewrite H2 by et); ss].
       eapply step_sem_cast; et. i. destruct optv; try sim_red;
-        try solve [eapply NEXT; i; clarify; unfold Cop.sem_binary_operation, Cop.sem_cmp; unfold Cop.sem_binarith; rewrite Heq;
+        try solve [eapplyf NEXT; i; clarify; unfold Cop.sem_binary_operation, Cop.sem_cmp; unfold Cop.sem_binarith; rewrite Heq;
                   try (erewrite H by et); try (erewrite H0 by et); try (erewrite H1 by et); try (erewrite H2 by et); ss].
       des_ifs; sim_red; 
-        eapply NEXT; i; clarify; unfold Cop.sem_binary_operation, Cop.sem_cmp; unfold Cop.sem_binarith; 
+        eapplyf NEXT; i; clarify; unfold Cop.sem_binary_operation, Cop.sem_cmp; unfold Cop.sem_binarith; 
           rewrite Heq in *; rewrite Heq0 in *;
             try (erewrite H by et); try (erewrite H0 by et); try (erewrite H1 by et); try (erewrite H2 by et); ss.
       all: unfold Val.of_bool; unfold Val.cmplu_bool; des_ifs; unfold Int64.cmpu; rewrite Heq1; ss.
     - des_ifs; unfold cmp_ptr_c; try sim_red; des_ifs_safe; 
-        try solve [unfold cmplu_bool_c; des_ifs; try sim_red; try eapply NEXT; i; ss; clarify; 
+        try solve [unfold cmplu_bool_c; des_ifs; try sim_red; try eapplyf NEXT; i; ss; clarify; 
                     unfold Cop.sem_cmp; rewrite Heq; unfold Cop.cmp_ptr; des_ifs_safe].
       + unfold cmplu_bool_c; des_ifs; try sim_red;
-          try solve [eapply NEXT; i; ss; clarify; unfold Cop.sem_cmp; rewrite Heq; unfold Cop.cmp_ptr; des_ifs_safe].
-          2,3: eapply step_weak_valid_pointer; et; i; des_ifs; sim_red; eapply NEXT; i; ss; clarify;
+          try solve [eapplyf NEXT; i; ss; clarify; unfold Cop.sem_cmp; rewrite Heq; unfold Cop.cmp_ptr; des_ifs_safe].
+          2,3: eapply step_weak_valid_pointer; et; i; des_ifs; sim_red; eapplyf NEXT; i; ss; clarify;
                 unfold Cop.sem_cmp; rewrite Heq; unfold Cop.cmp_ptr; ss; des_ifs_safe; 
                   unfold Mem.weak_valid_pointer in *; clarify.
-        * eapply NEXT; i; ss; clarify. unfold Cop.sem_cmp. rewrite Heq. unfold Cop.cmp_ptr. des_ifs_safe. ss.
+        * eapplyf NEXT; i; ss; clarify. unfold Cop.sem_cmp. rewrite Heq. unfold Cop.cmp_ptr. des_ifs_safe. ss.
           unfold Val.of_bool. des_ifs.
         * eapply step_weak_valid_pointer; et. i. sim_red. eapply step_weak_valid_pointer; et. i.
-          des_ifs; sim_red; eapply NEXT; i; ss; clarify;
+          des_ifs; sim_red; eapplyf NEXT; i; ss; clarify;
           unfold Cop.sem_cmp; rewrite Heq; unfold Cop.cmp_ptr; ss; des_ifs_safe; unfold Mem.weak_valid_pointer in *; clarify;
           unfold Val.of_bool; des_ifs. 
         * unfold ccallU. sim_red. ss. repeat (sim_tau; sim_red). unfold valid_pointerF. sim_red.
@@ -943,41 +947,41 @@ Section PROOF.
           unfold valid_pointerF. sim_red.
           repeat (sim_tau; sim_red). rewrite PSTATE. sim_red. repeat (sim_tau; sim_red).
           repeat match goal with | |- context [Mem.perm_dec ?x ?y ?z ?w ?a] => destruct (Mem.perm_dec x y z w a) end; sim_red;
-            eapply NEXT; i; ss; clarify;
+            eapplyf NEXT; i; ss; clarify;
               unfold Cop.sem_cmp; rewrite Heq; unfold Cop.cmp_ptr; ss; unfold Mem.valid_pointer in *;
                 destruct (eq_block _); des_ifs_safe;
           try solve [eapply map_blk_inj in e0; et; try contradiction];
           repeat (destruct (Mem.perm_dec _)); inv MM; unfold Mem.perm in *; ss.
       + unfold cmplu_bool_c; des_ifs; try sim_red;
-          try solve [eapply NEXT; i; ss; clarify; unfold Cop.sem_cmp; rewrite Heq; unfold Cop.cmp_ptr; des_ifs_safe].
-          2: eapply step_weak_valid_pointer; et; i; des_ifs; sim_red; eapply NEXT; i; ss; clarify;
+          try solve [eapplyf NEXT; i; ss; clarify; unfold Cop.sem_cmp; rewrite Heq; unfold Cop.cmp_ptr; des_ifs_safe].
+          2: eapply step_weak_valid_pointer; et; i; des_ifs; sim_red; eapplyf NEXT; i; ss; clarify;
                 unfold Cop.sem_cmp; rewrite Heq; unfold Cop.cmp_ptr; ss; des_ifs_safe; 
                   unfold Mem.weak_valid_pointer in *; clarify.
-          eapply NEXT; i; ss; clarify;
+          eapplyf NEXT; i; ss; clarify;
             unfold Cop.sem_cmp; rewrite Heq; unfold Cop.cmp_ptr; ss; unfold Mem.valid_pointer in *; des_ifs_safe.
           unfold Val.of_bool; ss. des_ifs.
       + unfold cmplu_bool_c; des_ifs; try sim_red;
-          try solve [eapply NEXT; i; ss; clarify; unfold Cop.sem_cmp; rewrite Heq; unfold Cop.cmp_ptr; des_ifs_safe].
-          1: eapply NEXT; i; ss; clarify; unfold Cop.sem_cmp; rewrite Heq; unfold Cop.cmp_ptr; des_ifs_safe.
-          2: eapply step_weak_valid_pointer; et; i; des_ifs; sim_red; eapply NEXT; i; ss; clarify;
+          try solve [eapplyf NEXT; i; ss; clarify; unfold Cop.sem_cmp; rewrite Heq; unfold Cop.cmp_ptr; des_ifs_safe].
+          1: eapplyf NEXT; i; ss; clarify; unfold Cop.sem_cmp; rewrite Heq; unfold Cop.cmp_ptr; des_ifs_safe.
+          2: eapply step_weak_valid_pointer; et; i; des_ifs; sim_red; eapplyf NEXT; i; ss; clarify;
                 unfold Cop.sem_cmp; rewrite Heq; unfold Cop.cmp_ptr; ss; des_ifs_safe; 
                   unfold Mem.weak_valid_pointer in *; clarify.
           all: unfold Val.of_bool; unfold Val.cmplu_bool; des_ifs; unfold Int64.cmpu; rewrite Heq1; ss.
       + unfold cmplu_bool_c; des_ifs; try sim_red;
-          try solve [eapply NEXT; i; ss; clarify; unfold Cop.sem_cmp; rewrite Heq; unfold Cop.cmp_ptr; des_ifs_safe].
-          2: eapply step_weak_valid_pointer; et; i; des_ifs; sim_red; eapply NEXT; i; ss; clarify;
+          try solve [eapplyf NEXT; i; ss; clarify; unfold Cop.sem_cmp; rewrite Heq; unfold Cop.cmp_ptr; des_ifs_safe].
+          2: eapply step_weak_valid_pointer; et; i; des_ifs; sim_red; eapplyf NEXT; i; ss; clarify;
                 unfold Cop.sem_cmp; rewrite Heq; unfold Cop.cmp_ptr; ss; des_ifs_safe; 
                   unfold Mem.weak_valid_pointer in *; clarify.
-          eapply NEXT; i; ss; clarify;
+          eapplyf NEXT; i; ss; clarify;
             unfold Cop.sem_cmp; rewrite Heq; unfold Cop.cmp_ptr; ss; unfold Mem.valid_pointer in *; des_ifs_safe.
           unfold Val.of_bool; ss. des_ifs.
       + unfold cmplu_bool_c; des_ifs; try sim_red;
-          try solve [eapply NEXT; i; ss; clarify; unfold Cop.sem_cmp; rewrite Heq; unfold Cop.cmp_ptr; des_ifs_safe].
-        * eapply step_weak_valid_pointer; et; i; des_ifs; sim_red; eapply NEXT; i; ss; clarify;
+          try solve [eapplyf NEXT; i; ss; clarify; unfold Cop.sem_cmp; rewrite Heq; unfold Cop.cmp_ptr; des_ifs_safe].
+        * eapply step_weak_valid_pointer; et; i; des_ifs; sim_red; eapplyf NEXT; i; ss; clarify;
                 unfold Cop.sem_cmp; rewrite Heq; unfold Cop.cmp_ptr; ss; des_ifs_safe; 
                   unfold Mem.weak_valid_pointer in *; clarify.
         * eapply step_weak_valid_pointer; et. i. sim_red. eapply step_weak_valid_pointer; et. i.
-          des_ifs; sim_red; eapply NEXT; i; ss; clarify;
+          des_ifs; sim_red; eapplyf NEXT; i; ss; clarify;
           unfold Cop.sem_cmp; rewrite Heq; unfold Cop.cmp_ptr; ss; des_ifs_safe; unfold Mem.weak_valid_pointer in *; clarify;
           unfold Val.of_bool; des_ifs. 
         * unfold ccallU. sim_red. ss. repeat (sim_tau; sim_red). unfold valid_pointerF. sim_red.
@@ -985,25 +989,25 @@ Section PROOF.
           unfold valid_pointerF. sim_red.
           repeat (sim_tau; sim_red). rewrite PSTATE. sim_red. repeat (sim_tau; sim_red).
           repeat match goal with | |- context [Mem.perm_dec ?x ?y ?z ?w ?a] => destruct (Mem.perm_dec x y z w a) end; sim_red;
-            eapply NEXT; i; ss; clarify;
+            eapplyf NEXT; i; ss; clarify;
               unfold Cop.sem_cmp; rewrite Heq; unfold Cop.cmp_ptr; ss; unfold Mem.valid_pointer in *;
                 destruct (eq_block _); des_ifs_safe;
           try solve [eapply map_blk_inj in e0; et; try contradiction];
           repeat (destruct (Mem.perm_dec _)); inv MM; unfold Mem.perm in *; ss.
       + unfold cmplu_bool_c; des_ifs; try sim_red;
-          try solve [eapply NEXT; i; ss; clarify; unfold Cop.sem_cmp; rewrite Heq; unfold Cop.cmp_ptr; des_ifs_safe].
-          1: eapply NEXT; i; ss; clarify; unfold Cop.sem_cmp; rewrite Heq; unfold Cop.cmp_ptr; des_ifs_safe.
-          2: eapply step_weak_valid_pointer; et; i; des_ifs; sim_red; eapply NEXT; i; ss; clarify;
+          try solve [eapplyf NEXT; i; ss; clarify; unfold Cop.sem_cmp; rewrite Heq; unfold Cop.cmp_ptr; des_ifs_safe].
+          1: eapplyf NEXT; i; ss; clarify; unfold Cop.sem_cmp; rewrite Heq; unfold Cop.cmp_ptr; des_ifs_safe.
+          2: eapply step_weak_valid_pointer; et; i; des_ifs; sim_red; eapplyf NEXT; i; ss; clarify;
                 unfold Cop.sem_cmp; rewrite Heq; unfold Cop.cmp_ptr; ss; des_ifs_safe; 
                   unfold Mem.weak_valid_pointer in *; clarify.
           all: unfold Val.of_bool; unfold Val.cmplu_bool; des_ifs; unfold Int64.cmpu; rewrite Heq1; ss.
       + unfold cmplu_bool_c; des_ifs; try sim_red;
-          try solve [eapply NEXT; i; ss; clarify; unfold Cop.sem_cmp; rewrite Heq; unfold Cop.cmp_ptr; des_ifs_safe].
-        * eapply step_weak_valid_pointer; et; i; des_ifs; sim_red; eapply NEXT; i; ss; clarify;
+          try solve [eapplyf NEXT; i; ss; clarify; unfold Cop.sem_cmp; rewrite Heq; unfold Cop.cmp_ptr; des_ifs_safe].
+        * eapply step_weak_valid_pointer; et; i; des_ifs; sim_red; eapplyf NEXT; i; ss; clarify;
                 unfold Cop.sem_cmp; rewrite Heq; unfold Cop.cmp_ptr; ss; des_ifs_safe; 
                   unfold Mem.weak_valid_pointer in *; clarify.
         * eapply step_weak_valid_pointer; et. i. sim_red. eapply step_weak_valid_pointer; et. i.
-          des_ifs; sim_red; eapply NEXT; i; ss; clarify;
+          des_ifs; sim_red; eapplyf NEXT; i; ss; clarify;
           unfold Cop.sem_cmp; rewrite Heq; unfold Cop.cmp_ptr; ss; des_ifs_safe; unfold Mem.weak_valid_pointer in *; clarify;
           unfold Val.of_bool; des_ifs. 
         * unfold ccallU. sim_red. ss. repeat (sim_tau; sim_red). unfold valid_pointerF. sim_red.
@@ -1011,34 +1015,34 @@ Section PROOF.
           unfold valid_pointerF. sim_red.
           repeat (sim_tau; sim_red). rewrite PSTATE. sim_red. repeat (sim_tau; sim_red).
           repeat match goal with | |- context [Mem.perm_dec ?x ?y ?z ?w ?a] => destruct (Mem.perm_dec x y z w a) end; sim_red;
-            eapply NEXT; i; ss; clarify;
+            eapplyf NEXT; i; ss; clarify;
               unfold Cop.sem_cmp; rewrite Heq; unfold Cop.cmp_ptr; ss; unfold Mem.valid_pointer in *;
                 destruct (eq_block _); des_ifs_safe;
           try solve [eapply map_blk_inj in e0; et; try contradiction];
           repeat (destruct (Mem.perm_dec _)); inv MM; unfold Mem.perm in *; ss.
     + unfold sem_binarith_c. sim_red. eapply step_sem_cast; et. i. destruct optv; sim_red;
-        try solve [ eapply NEXT; i; clarify; unfold Cop.sem_binary_operation, Cop.sem_cmp; unfold Cop.sem_binarith; rewrite Heq;
+        try solve [ eapplyf NEXT; i; clarify; unfold Cop.sem_binary_operation, Cop.sem_cmp; unfold Cop.sem_binarith; rewrite Heq;
                   try (erewrite H by et); try (erewrite H0 by et); try (erewrite H1 by et); try (erewrite H2 by et); ss].
       eapply step_sem_cast; et. i. destruct optv; try sim_red;
-        try solve [eapply NEXT; i; clarify; unfold Cop.sem_binary_operation, Cop.sem_cmp; unfold Cop.sem_binarith; rewrite Heq;
+        try solve [eapplyf NEXT; i; clarify; unfold Cop.sem_binary_operation, Cop.sem_cmp; unfold Cop.sem_binarith; rewrite Heq;
                   try (erewrite H by et); try (erewrite H0 by et); try (erewrite H1 by et); try (erewrite H2 by et); ss].
       des_ifs; sim_red; 
-        eapply NEXT; i; clarify; unfold Cop.sem_binary_operation, Cop.sem_cmp; unfold Cop.sem_binarith; 
+        eapplyf NEXT; i; clarify; unfold Cop.sem_binary_operation, Cop.sem_cmp; unfold Cop.sem_binarith; 
           rewrite Heq in *; rewrite Heq0 in *;
             try (erewrite H by et); try (erewrite H0 by et); try (erewrite H1 by et); try (erewrite H2 by et); ss.
       all: unfold Val.of_bool; unfold Val.cmplu_bool; des_ifs; unfold Int64.cmpu; rewrite Heq1; ss.
     - des_ifs; unfold cmp_ptr_c; try sim_red; des_ifs_safe; 
-        try solve [unfold cmplu_bool_c; des_ifs; try sim_red; try eapply NEXT; i; ss; clarify; 
+        try solve [unfold cmplu_bool_c; des_ifs; try sim_red; try eapplyf NEXT; i; ss; clarify; 
                     unfold Cop.sem_cmp; rewrite Heq; unfold Cop.cmp_ptr; des_ifs_safe].
       + unfold cmplu_bool_c; des_ifs; try sim_red;
-          try solve [eapply NEXT; i; ss; clarify; unfold Cop.sem_cmp; rewrite Heq; unfold Cop.cmp_ptr; des_ifs_safe].
-          2,3: eapply step_weak_valid_pointer; et; i; des_ifs; sim_red; eapply NEXT; i; ss; clarify;
+          try solve [eapplyf NEXT; i; ss; clarify; unfold Cop.sem_cmp; rewrite Heq; unfold Cop.cmp_ptr; des_ifs_safe].
+          2,3: eapply step_weak_valid_pointer; et; i; des_ifs; sim_red; eapplyf NEXT; i; ss; clarify;
                 unfold Cop.sem_cmp; rewrite Heq; unfold Cop.cmp_ptr; ss; des_ifs_safe; 
                   unfold Mem.weak_valid_pointer in *; clarify.
-        * eapply NEXT; i; ss; clarify. unfold Cop.sem_cmp. rewrite Heq. unfold Cop.cmp_ptr. des_ifs_safe. ss.
+        * eapplyf NEXT; i; ss; clarify. unfold Cop.sem_cmp. rewrite Heq. unfold Cop.cmp_ptr. des_ifs_safe. ss.
           unfold Val.of_bool. des_ifs.
         * eapply step_weak_valid_pointer; et. i. sim_red. eapply step_weak_valid_pointer; et. i.
-          des_ifs; sim_red; eapply NEXT; i; ss; clarify;
+          des_ifs; sim_red; eapplyf NEXT; i; ss; clarify;
           unfold Cop.sem_cmp; rewrite Heq; unfold Cop.cmp_ptr; ss; des_ifs_safe; unfold Mem.weak_valid_pointer in *; clarify;
           unfold Val.of_bool; des_ifs. 
         * unfold ccallU. sim_red. ss. repeat (sim_tau; sim_red). unfold valid_pointerF. sim_red.
@@ -1046,41 +1050,41 @@ Section PROOF.
           unfold valid_pointerF. sim_red.
           repeat (sim_tau; sim_red). rewrite PSTATE. sim_red. repeat (sim_tau; sim_red).
           repeat match goal with | |- context [Mem.perm_dec ?x ?y ?z ?w ?a] => destruct (Mem.perm_dec x y z w a) end; sim_red;
-            eapply NEXT; i; ss; clarify;
+            eapplyf NEXT; i; ss; clarify;
               unfold Cop.sem_cmp; rewrite Heq; unfold Cop.cmp_ptr; ss; unfold Mem.valid_pointer in *;
                 destruct (eq_block _); des_ifs_safe;
           try solve [eapply map_blk_inj in e0; et; try contradiction];
           repeat (destruct (Mem.perm_dec _)); inv MM; unfold Mem.perm in *; ss.
       + unfold cmplu_bool_c; des_ifs; try sim_red;
-          try solve [eapply NEXT; i; ss; clarify; unfold Cop.sem_cmp; rewrite Heq; unfold Cop.cmp_ptr; des_ifs_safe].
-          2: eapply step_weak_valid_pointer; et; i; des_ifs; sim_red; eapply NEXT; i; ss; clarify;
+          try solve [eapplyf NEXT; i; ss; clarify; unfold Cop.sem_cmp; rewrite Heq; unfold Cop.cmp_ptr; des_ifs_safe].
+          2: eapply step_weak_valid_pointer; et; i; des_ifs; sim_red; eapplyf NEXT; i; ss; clarify;
                 unfold Cop.sem_cmp; rewrite Heq; unfold Cop.cmp_ptr; ss; des_ifs_safe; 
                   unfold Mem.weak_valid_pointer in *; clarify.
-          eapply NEXT; i; ss; clarify;
+          eapplyf NEXT; i; ss; clarify;
             unfold Cop.sem_cmp; rewrite Heq; unfold Cop.cmp_ptr; ss; unfold Mem.valid_pointer in *; des_ifs_safe.
           unfold Val.of_bool; ss. des_ifs.
       + unfold cmplu_bool_c; des_ifs; try sim_red;
-          try solve [eapply NEXT; i; ss; clarify; unfold Cop.sem_cmp; rewrite Heq; unfold Cop.cmp_ptr; des_ifs_safe].
-          1: eapply NEXT; i; ss; clarify; unfold Cop.sem_cmp; rewrite Heq; unfold Cop.cmp_ptr; des_ifs_safe.
-          2: eapply step_weak_valid_pointer; et; i; des_ifs; sim_red; eapply NEXT; i; ss; clarify;
+          try solve [eapplyf NEXT; i; ss; clarify; unfold Cop.sem_cmp; rewrite Heq; unfold Cop.cmp_ptr; des_ifs_safe].
+          1: eapplyf NEXT; i; ss; clarify; unfold Cop.sem_cmp; rewrite Heq; unfold Cop.cmp_ptr; des_ifs_safe.
+          2: eapply step_weak_valid_pointer; et; i; des_ifs; sim_red; eapplyf NEXT; i; ss; clarify;
                 unfold Cop.sem_cmp; rewrite Heq; unfold Cop.cmp_ptr; ss; des_ifs_safe; 
                   unfold Mem.weak_valid_pointer in *; clarify.
           all: unfold Val.of_bool; unfold Val.cmplu_bool; des_ifs; unfold Int64.cmpu; rewrite Heq1; ss.
       + unfold cmplu_bool_c; des_ifs; try sim_red;
-          try solve [eapply NEXT; i; ss; clarify; unfold Cop.sem_cmp; rewrite Heq; unfold Cop.cmp_ptr; des_ifs_safe].
-          2: eapply step_weak_valid_pointer; et; i; des_ifs; sim_red; eapply NEXT; i; ss; clarify;
+          try solve [eapplyf NEXT; i; ss; clarify; unfold Cop.sem_cmp; rewrite Heq; unfold Cop.cmp_ptr; des_ifs_safe].
+          2: eapply step_weak_valid_pointer; et; i; des_ifs; sim_red; eapplyf NEXT; i; ss; clarify;
                 unfold Cop.sem_cmp; rewrite Heq; unfold Cop.cmp_ptr; ss; des_ifs_safe; 
                   unfold Mem.weak_valid_pointer in *; clarify.
-          eapply NEXT; i; ss; clarify;
+          eapplyf NEXT; i; ss; clarify;
             unfold Cop.sem_cmp; rewrite Heq; unfold Cop.cmp_ptr; ss; unfold Mem.valid_pointer in *; des_ifs_safe.
           unfold Val.of_bool; ss. des_ifs.
       + unfold cmplu_bool_c; des_ifs; try sim_red;
-          try solve [eapply NEXT; i; ss; clarify; unfold Cop.sem_cmp; rewrite Heq; unfold Cop.cmp_ptr; des_ifs_safe].
-        * eapply step_weak_valid_pointer; et; i; des_ifs; sim_red; eapply NEXT; i; ss; clarify;
+          try solve [eapplyf NEXT; i; ss; clarify; unfold Cop.sem_cmp; rewrite Heq; unfold Cop.cmp_ptr; des_ifs_safe].
+        * eapply step_weak_valid_pointer; et; i; des_ifs; sim_red; eapplyf NEXT; i; ss; clarify;
                 unfold Cop.sem_cmp; rewrite Heq; unfold Cop.cmp_ptr; ss; des_ifs_safe; 
                   unfold Mem.weak_valid_pointer in *; clarify.
         * eapply step_weak_valid_pointer; et. i. sim_red. eapply step_weak_valid_pointer; et. i.
-          des_ifs; sim_red; eapply NEXT; i; ss; clarify;
+          des_ifs; sim_red; eapplyf NEXT; i; ss; clarify;
           unfold Cop.sem_cmp; rewrite Heq; unfold Cop.cmp_ptr; ss; des_ifs_safe; unfold Mem.weak_valid_pointer in *; clarify;
           unfold Val.of_bool; des_ifs. 
         * unfold ccallU. sim_red. ss. repeat (sim_tau; sim_red). unfold valid_pointerF. sim_red.
@@ -1088,25 +1092,25 @@ Section PROOF.
           unfold valid_pointerF. sim_red.
           repeat (sim_tau; sim_red). rewrite PSTATE. sim_red. repeat (sim_tau; sim_red).
           repeat match goal with | |- context [Mem.perm_dec ?x ?y ?z ?w ?a] => destruct (Mem.perm_dec x y z w a) end; sim_red;
-            eapply NEXT; i; ss; clarify;
+            eapplyf NEXT; i; ss; clarify;
               unfold Cop.sem_cmp; rewrite Heq; unfold Cop.cmp_ptr; ss; unfold Mem.valid_pointer in *;
                 destruct (eq_block _); des_ifs_safe;
           try solve [eapply map_blk_inj in e0; et; try contradiction];
           repeat (destruct (Mem.perm_dec _)); inv MM; unfold Mem.perm in *; ss.
       + unfold cmplu_bool_c; des_ifs; try sim_red;
-          try solve [eapply NEXT; i; ss; clarify; unfold Cop.sem_cmp; rewrite Heq; unfold Cop.cmp_ptr; des_ifs_safe].
-          1: eapply NEXT; i; ss; clarify; unfold Cop.sem_cmp; rewrite Heq; unfold Cop.cmp_ptr; des_ifs_safe.
-          2: eapply step_weak_valid_pointer; et; i; des_ifs; sim_red; eapply NEXT; i; ss; clarify;
+          try solve [eapplyf NEXT; i; ss; clarify; unfold Cop.sem_cmp; rewrite Heq; unfold Cop.cmp_ptr; des_ifs_safe].
+          1: eapplyf NEXT; i; ss; clarify; unfold Cop.sem_cmp; rewrite Heq; unfold Cop.cmp_ptr; des_ifs_safe.
+          2: eapply step_weak_valid_pointer; et; i; des_ifs; sim_red; eapplyf NEXT; i; ss; clarify;
                 unfold Cop.sem_cmp; rewrite Heq; unfold Cop.cmp_ptr; ss; des_ifs_safe; 
                   unfold Mem.weak_valid_pointer in *; clarify.
           all: unfold Val.of_bool; unfold Val.cmplu_bool; des_ifs; unfold Int64.cmpu; rewrite Heq1; ss.
       + unfold cmplu_bool_c; des_ifs; try sim_red;
-          try solve [eapply NEXT; i; ss; clarify; unfold Cop.sem_cmp; rewrite Heq; unfold Cop.cmp_ptr; des_ifs_safe].
-        * eapply step_weak_valid_pointer; et; i; des_ifs; sim_red; eapply NEXT; i; ss; clarify;
+          try solve [eapplyf NEXT; i; ss; clarify; unfold Cop.sem_cmp; rewrite Heq; unfold Cop.cmp_ptr; des_ifs_safe].
+        * eapply step_weak_valid_pointer; et; i; des_ifs; sim_red; eapplyf NEXT; i; ss; clarify;
                 unfold Cop.sem_cmp; rewrite Heq; unfold Cop.cmp_ptr; ss; des_ifs_safe; 
                   unfold Mem.weak_valid_pointer in *; clarify.
         * eapply step_weak_valid_pointer; et. i. sim_red. eapply step_weak_valid_pointer; et. i.
-          des_ifs; sim_red; eapply NEXT; i; ss; clarify;
+          des_ifs; sim_red; eapplyf NEXT; i; ss; clarify;
           unfold Cop.sem_cmp; rewrite Heq; unfold Cop.cmp_ptr; ss; des_ifs_safe; unfold Mem.weak_valid_pointer in *; clarify;
           unfold Val.of_bool; des_ifs. 
         * unfold ccallU. sim_red. ss. repeat (sim_tau; sim_red). unfold valid_pointerF. sim_red.
@@ -1114,34 +1118,34 @@ Section PROOF.
           unfold valid_pointerF. sim_red.
           repeat (sim_tau; sim_red). rewrite PSTATE. sim_red. repeat (sim_tau; sim_red).
           repeat match goal with | |- context [Mem.perm_dec ?x ?y ?z ?w ?a] => destruct (Mem.perm_dec x y z w a) end; sim_red;
-            eapply NEXT; i; ss; clarify;
+            eapplyf NEXT; i; ss; clarify;
               unfold Cop.sem_cmp; rewrite Heq; unfold Cop.cmp_ptr; ss; unfold Mem.valid_pointer in *;
                 destruct (eq_block _); des_ifs_safe;
           try solve [eapply map_blk_inj in e0; et; try contradiction];
           repeat (destruct (Mem.perm_dec _)); inv MM; unfold Mem.perm in *; ss.
     + unfold sem_binarith_c. sim_red. eapply step_sem_cast; et. i. destruct optv; sim_red;
-        try solve [ eapply NEXT; i; clarify; unfold Cop.sem_binary_operation, Cop.sem_cmp; unfold Cop.sem_binarith; rewrite Heq;
+        try solve [ eapplyf NEXT; i; clarify; unfold Cop.sem_binary_operation, Cop.sem_cmp; unfold Cop.sem_binarith; rewrite Heq;
                   try (erewrite H by et); try (erewrite H0 by et); try (erewrite H1 by et); try (erewrite H2 by et); ss].
       eapply step_sem_cast; et. i. destruct optv; try sim_red;
-        try solve [eapply NEXT; i; clarify; unfold Cop.sem_binary_operation, Cop.sem_cmp; unfold Cop.sem_binarith; rewrite Heq;
+        try solve [eapplyf NEXT; i; clarify; unfold Cop.sem_binary_operation, Cop.sem_cmp; unfold Cop.sem_binarith; rewrite Heq;
                   try (erewrite H by et); try (erewrite H0 by et); try (erewrite H1 by et); try (erewrite H2 by et); ss].
       des_ifs; sim_red; 
-        eapply NEXT; i; clarify; unfold Cop.sem_binary_operation, Cop.sem_cmp; unfold Cop.sem_binarith; 
+        eapplyf NEXT; i; clarify; unfold Cop.sem_binary_operation, Cop.sem_cmp; unfold Cop.sem_binarith; 
           rewrite Heq in *; rewrite Heq0 in *;
             try (erewrite H by et); try (erewrite H0 by et); try (erewrite H1 by et); try (erewrite H2 by et); ss.
       all: unfold Val.of_bool; unfold Val.cmplu_bool; des_ifs; unfold Int64.cmpu; rewrite Heq1; ss.
     - des_ifs; unfold cmp_ptr_c; try sim_red; des_ifs_safe; 
-        try solve [unfold cmplu_bool_c; des_ifs; try sim_red; try eapply NEXT; i; ss; clarify; 
+        try solve [unfold cmplu_bool_c; des_ifs; try sim_red; try eapplyf NEXT; i; ss; clarify; 
                     unfold Cop.sem_cmp; rewrite Heq; unfold Cop.cmp_ptr; des_ifs_safe].
       + unfold cmplu_bool_c; des_ifs; try sim_red;
-          try solve [eapply NEXT; i; ss; clarify; unfold Cop.sem_cmp; rewrite Heq; unfold Cop.cmp_ptr; des_ifs_safe].
-          2,3: eapply step_weak_valid_pointer; et; i; des_ifs; sim_red; eapply NEXT; i; ss; clarify;
+          try solve [eapplyf NEXT; i; ss; clarify; unfold Cop.sem_cmp; rewrite Heq; unfold Cop.cmp_ptr; des_ifs_safe].
+          2,3: eapply step_weak_valid_pointer; et; i; des_ifs; sim_red; eapplyf NEXT; i; ss; clarify;
                 unfold Cop.sem_cmp; rewrite Heq; unfold Cop.cmp_ptr; ss; des_ifs_safe; 
                   unfold Mem.weak_valid_pointer in *; clarify.
-        * eapply NEXT; i; ss; clarify. unfold Cop.sem_cmp. rewrite Heq. unfold Cop.cmp_ptr. des_ifs_safe. ss.
+        * eapplyf NEXT; i; ss; clarify. unfold Cop.sem_cmp. rewrite Heq. unfold Cop.cmp_ptr. des_ifs_safe. ss.
           unfold Val.of_bool. des_ifs.
         * eapply step_weak_valid_pointer; et. i. sim_red. eapply step_weak_valid_pointer; et. i.
-          des_ifs; sim_red; eapply NEXT; i; ss; clarify;
+          des_ifs; sim_red; eapplyf NEXT; i; ss; clarify;
           unfold Cop.sem_cmp; rewrite Heq; unfold Cop.cmp_ptr; ss; des_ifs_safe; unfold Mem.weak_valid_pointer in *; clarify;
           unfold Val.of_bool; des_ifs. 
         * unfold ccallU. sim_red. ss. repeat (sim_tau; sim_red). unfold valid_pointerF. sim_red.
@@ -1149,41 +1153,41 @@ Section PROOF.
           unfold valid_pointerF. sim_red.
           repeat (sim_tau; sim_red). rewrite PSTATE. sim_red. repeat (sim_tau; sim_red).
           repeat match goal with | |- context [Mem.perm_dec ?x ?y ?z ?w ?a] => destruct (Mem.perm_dec x y z w a) end; sim_red;
-            eapply NEXT; i; ss; clarify;
+            eapplyf NEXT; i; ss; clarify;
               unfold Cop.sem_cmp; rewrite Heq; unfold Cop.cmp_ptr; ss; unfold Mem.valid_pointer in *;
                 destruct (eq_block _); des_ifs_safe;
           try solve [eapply map_blk_inj in e0; et; try contradiction];
           repeat (destruct (Mem.perm_dec _)); inv MM; unfold Mem.perm in *; ss.
       + unfold cmplu_bool_c; des_ifs; try sim_red;
-          try solve [eapply NEXT; i; ss; clarify; unfold Cop.sem_cmp; rewrite Heq; unfold Cop.cmp_ptr; des_ifs_safe].
-          2: eapply step_weak_valid_pointer; et; i; des_ifs; sim_red; eapply NEXT; i; ss; clarify;
+          try solve [eapplyf NEXT; i; ss; clarify; unfold Cop.sem_cmp; rewrite Heq; unfold Cop.cmp_ptr; des_ifs_safe].
+          2: eapply step_weak_valid_pointer; et; i; des_ifs; sim_red; eapplyf NEXT; i; ss; clarify;
                 unfold Cop.sem_cmp; rewrite Heq; unfold Cop.cmp_ptr; ss; des_ifs_safe; 
                   unfold Mem.weak_valid_pointer in *; clarify.
-          eapply NEXT; i; ss; clarify;
+          eapplyf NEXT; i; ss; clarify;
             unfold Cop.sem_cmp; rewrite Heq; unfold Cop.cmp_ptr; ss; unfold Mem.valid_pointer in *; des_ifs_safe.
           unfold Val.of_bool; ss. des_ifs.
       + unfold cmplu_bool_c; des_ifs; try sim_red;
-          try solve [eapply NEXT; i; ss; clarify; unfold Cop.sem_cmp; rewrite Heq; unfold Cop.cmp_ptr; des_ifs_safe].
-          1: eapply NEXT; i; ss; clarify; unfold Cop.sem_cmp; rewrite Heq; unfold Cop.cmp_ptr; des_ifs_safe.
-          2: eapply step_weak_valid_pointer; et; i; des_ifs; sim_red; eapply NEXT; i; ss; clarify;
+          try solve [eapplyf NEXT; i; ss; clarify; unfold Cop.sem_cmp; rewrite Heq; unfold Cop.cmp_ptr; des_ifs_safe].
+          1: eapplyf NEXT; i; ss; clarify; unfold Cop.sem_cmp; rewrite Heq; unfold Cop.cmp_ptr; des_ifs_safe.
+          2: eapply step_weak_valid_pointer; et; i; des_ifs; sim_red; eapplyf NEXT; i; ss; clarify;
                 unfold Cop.sem_cmp; rewrite Heq; unfold Cop.cmp_ptr; ss; des_ifs_safe; 
                   unfold Mem.weak_valid_pointer in *; clarify.
           all: unfold Val.of_bool; unfold Val.cmplu_bool; des_ifs; unfold Int64.cmpu; rewrite Heq1; ss.
       + unfold cmplu_bool_c; des_ifs; try sim_red;
-          try solve [eapply NEXT; i; ss; clarify; unfold Cop.sem_cmp; rewrite Heq; unfold Cop.cmp_ptr; des_ifs_safe].
-          2: eapply step_weak_valid_pointer; et; i; des_ifs; sim_red; eapply NEXT; i; ss; clarify;
+          try solve [eapplyf NEXT; i; ss; clarify; unfold Cop.sem_cmp; rewrite Heq; unfold Cop.cmp_ptr; des_ifs_safe].
+          2: eapply step_weak_valid_pointer; et; i; des_ifs; sim_red; eapplyf NEXT; i; ss; clarify;
                 unfold Cop.sem_cmp; rewrite Heq; unfold Cop.cmp_ptr; ss; des_ifs_safe; 
                   unfold Mem.weak_valid_pointer in *; clarify.
-          eapply NEXT; i; ss; clarify;
+          eapplyf NEXT; i; ss; clarify;
             unfold Cop.sem_cmp; rewrite Heq; unfold Cop.cmp_ptr; ss; unfold Mem.valid_pointer in *; des_ifs_safe.
           unfold Val.of_bool; ss. des_ifs.
       + unfold cmplu_bool_c; des_ifs; try sim_red;
-          try solve [eapply NEXT; i; ss; clarify; unfold Cop.sem_cmp; rewrite Heq; unfold Cop.cmp_ptr; des_ifs_safe].
-        * eapply step_weak_valid_pointer; et; i; des_ifs; sim_red; eapply NEXT; i; ss; clarify;
+          try solve [eapplyf NEXT; i; ss; clarify; unfold Cop.sem_cmp; rewrite Heq; unfold Cop.cmp_ptr; des_ifs_safe].
+        * eapply step_weak_valid_pointer; et; i; des_ifs; sim_red; eapplyf NEXT; i; ss; clarify;
                 unfold Cop.sem_cmp; rewrite Heq; unfold Cop.cmp_ptr; ss; des_ifs_safe; 
                   unfold Mem.weak_valid_pointer in *; clarify.
         * eapply step_weak_valid_pointer; et. i. sim_red. eapply step_weak_valid_pointer; et. i.
-          des_ifs; sim_red; eapply NEXT; i; ss; clarify;
+          des_ifs; sim_red; eapplyf NEXT; i; ss; clarify;
           unfold Cop.sem_cmp; rewrite Heq; unfold Cop.cmp_ptr; ss; des_ifs_safe; unfold Mem.weak_valid_pointer in *; clarify;
           unfold Val.of_bool; des_ifs. 
         * unfold ccallU. sim_red. ss. repeat (sim_tau; sim_red). unfold valid_pointerF. sim_red.
@@ -1191,25 +1195,25 @@ Section PROOF.
           unfold valid_pointerF. sim_red.
           repeat (sim_tau; sim_red). rewrite PSTATE. sim_red. repeat (sim_tau; sim_red).
           repeat match goal with | |- context [Mem.perm_dec ?x ?y ?z ?w ?a] => destruct (Mem.perm_dec x y z w a) end; sim_red;
-            eapply NEXT; i; ss; clarify;
+            eapplyf NEXT; i; ss; clarify;
               unfold Cop.sem_cmp; rewrite Heq; unfold Cop.cmp_ptr; ss; unfold Mem.valid_pointer in *;
                 destruct (eq_block _); des_ifs_safe;
           try solve [eapply map_blk_inj in e0; et; try contradiction];
           repeat (destruct (Mem.perm_dec _)); inv MM; unfold Mem.perm in *; ss.
       + unfold cmplu_bool_c; des_ifs; try sim_red;
-          try solve [eapply NEXT; i; ss; clarify; unfold Cop.sem_cmp; rewrite Heq; unfold Cop.cmp_ptr; des_ifs_safe].
-          1: eapply NEXT; i; ss; clarify; unfold Cop.sem_cmp; rewrite Heq; unfold Cop.cmp_ptr; des_ifs_safe.
-          2: eapply step_weak_valid_pointer; et; i; des_ifs; sim_red; eapply NEXT; i; ss; clarify;
+          try solve [eapplyf NEXT; i; ss; clarify; unfold Cop.sem_cmp; rewrite Heq; unfold Cop.cmp_ptr; des_ifs_safe].
+          1: eapplyf NEXT; i; ss; clarify; unfold Cop.sem_cmp; rewrite Heq; unfold Cop.cmp_ptr; des_ifs_safe.
+          2: eapply step_weak_valid_pointer; et; i; des_ifs; sim_red; eapplyf NEXT; i; ss; clarify;
                 unfold Cop.sem_cmp; rewrite Heq; unfold Cop.cmp_ptr; ss; des_ifs_safe; 
                   unfold Mem.weak_valid_pointer in *; clarify.
           all: unfold Val.of_bool; unfold Val.cmplu_bool; des_ifs; unfold Int64.cmpu; rewrite Heq1; ss.
       + unfold cmplu_bool_c; des_ifs; try sim_red;
-          try solve [eapply NEXT; i; ss; clarify; unfold Cop.sem_cmp; rewrite Heq; unfold Cop.cmp_ptr; des_ifs_safe].
-        * eapply step_weak_valid_pointer; et; i; des_ifs; sim_red; eapply NEXT; i; ss; clarify;
+          try solve [eapplyf NEXT; i; ss; clarify; unfold Cop.sem_cmp; rewrite Heq; unfold Cop.cmp_ptr; des_ifs_safe].
+        * eapply step_weak_valid_pointer; et; i; des_ifs; sim_red; eapplyf NEXT; i; ss; clarify;
                 unfold Cop.sem_cmp; rewrite Heq; unfold Cop.cmp_ptr; ss; des_ifs_safe; 
                   unfold Mem.weak_valid_pointer in *; clarify.
         * eapply step_weak_valid_pointer; et. i. sim_red. eapply step_weak_valid_pointer; et. i.
-          des_ifs; sim_red; eapply NEXT; i; ss; clarify;
+          des_ifs; sim_red; eapplyf NEXT; i; ss; clarify;
           unfold Cop.sem_cmp; rewrite Heq; unfold Cop.cmp_ptr; ss; des_ifs_safe; unfold Mem.weak_valid_pointer in *; clarify;
           unfold Val.of_bool; des_ifs. 
         * unfold ccallU. sim_red. ss. repeat (sim_tau; sim_red). unfold valid_pointerF. sim_red.
@@ -1217,19 +1221,19 @@ Section PROOF.
           unfold valid_pointerF. sim_red.
           repeat (sim_tau; sim_red). rewrite PSTATE. sim_red. repeat (sim_tau; sim_red).
           repeat match goal with | |- context [Mem.perm_dec ?x ?y ?z ?w ?a] => destruct (Mem.perm_dec x y z w a) end; sim_red;
-            eapply NEXT; i; ss; clarify;
+            eapplyf NEXT; i; ss; clarify;
               unfold Cop.sem_cmp; rewrite Heq; unfold Cop.cmp_ptr; ss; unfold Mem.valid_pointer in *;
                 destruct (eq_block _); des_ifs_safe;
           try solve [eapply map_blk_inj in e0; et; try contradiction];
           repeat (destruct (Mem.perm_dec _)); inv MM; unfold Mem.perm in *; ss.
     + unfold sem_binarith_c. sim_red. eapply step_sem_cast; et. i. destruct optv; sim_red;
-        try solve [ eapply NEXT; i; clarify; unfold Cop.sem_binary_operation, Cop.sem_cmp; unfold Cop.sem_binarith; rewrite Heq;
+        try solve [ eapplyf NEXT; i; clarify; unfold Cop.sem_binary_operation, Cop.sem_cmp; unfold Cop.sem_binarith; rewrite Heq;
                   try (erewrite H by et); try (erewrite H0 by et); try (erewrite H1 by et); try (erewrite H2 by et); ss].
       eapply step_sem_cast; et. i. destruct optv; try sim_red;
-        try solve [eapply NEXT; i; clarify; unfold Cop.sem_binary_operation, Cop.sem_cmp; unfold Cop.sem_binarith; rewrite Heq;
+        try solve [eapplyf NEXT; i; clarify; unfold Cop.sem_binary_operation, Cop.sem_cmp; unfold Cop.sem_binarith; rewrite Heq;
                   try (erewrite H by et); try (erewrite H0 by et); try (erewrite H1 by et); try (erewrite H2 by et); ss].
       des_ifs; sim_red; 
-        eapply NEXT; i; clarify; unfold Cop.sem_binary_operation, Cop.sem_cmp; unfold Cop.sem_binarith; 
+        eapplyf NEXT; i; clarify; unfold Cop.sem_binary_operation, Cop.sem_cmp; unfold Cop.sem_binarith; 
           rewrite Heq in *; rewrite Heq0 in *;
             try (erewrite H by et); try (erewrite H0 by et); try (erewrite H1 by et); try (erewrite H2 by et); ss.
       all: unfold Val.of_bool; unfold Val.cmplu_bool; des_ifs; unfold Int64.cmpu; rewrite Heq1; ss.
